work on sn

Common/Term.lean
@@ -37,37 +37,37 @@ instance Const_inst_LawfulBEq : LawfulBEq Const where
   eq_of_beq := by intro m1 m2 h; cases m1 <;> cases m2 <;> simp at *
   rfl := by intro m; cases m <;> simp
 
-inductive CvTerm : Type where
-| sym : CvTerm -> CvTerm
-| trans : CvTerm -> CvTerm -> CvTerm
-| none : CvTerm
-| const : CvTerm
-| bound : Nat -> CvTerm
-| all_congr : CvTerm -> CvTerm -> CvTerm
-| lam_congr : CvTerm -> CvTerm -> CvTerm
-| lam_eta : CvTerm -> CvTerm
-| lam_mf_erased : CvTerm -> CvTerm
-| lam_m0_erased : CvTerm -> CvTerm
-| app_congr : CvTerm -> CvTerm -> CvTerm
-| app_beta : CvTerm -> CvTerm
-| app_m0_erased : CvTerm -> CvTerm
-| prod_congr : CvTerm -> CvTerm -> CvTerm
-| pair_congr : CvTerm -> CvTerm -> CvTerm -> CvTerm
-| pair_erased : CvTerm -> CvTerm
-| fst_congr : CvTerm -> CvTerm
-| fst_erased : CvTerm -> CvTerm
-| snd_congr : CvTerm -> CvTerm
-| snd_erased : CvTerm -> CvTerm
-| phi_congr : CvTerm -> CvTerm -> CvTerm -> CvTerm
-| phi_erased : CvTerm -> CvTerm
-| eq_congr : CvTerm -> CvTerm -> CvTerm -> CvTerm
-| refl_congr : CvTerm -> CvTerm
-| refl_erased : CvTerm -> CvTerm
-| subst_congr : CvTerm -> CvTerm -> CvTerm
-| subst_erased : CvTerm -> CvTerm
-| conv_congr : CvTerm -> CvTerm -> CvTerm
-| conv_erased : CvTerm -> CvTerm
-deriving BEq
+-- inductive CvTerm : Type where
+-- | sym : CvTerm -> CvTerm
+-- | trans : CvTerm -> CvTerm -> CvTerm
+-- | none : CvTerm
+-- | const : CvTerm
+-- | bound : Nat -> CvTerm
+-- | all_congr : CvTerm -> CvTerm -> CvTerm
+-- | lam_congr : CvTerm -> CvTerm -> CvTerm
+-- | lam_eta : CvTerm -> CvTerm
+-- | lam_mf_erased : CvTerm -> CvTerm
+-- | lam_m0_erased : CvTerm -> CvTerm
+-- | app_congr : CvTerm -> CvTerm -> CvTerm
+-- | app_beta : CvTerm -> CvTerm
+-- | app_m0_erased : CvTerm -> CvTerm
+-- | prod_congr : CvTerm -> CvTerm -> CvTerm
+-- | pair_congr : CvTerm -> CvTerm -> CvTerm -> CvTerm
+-- | pair_erased : CvTerm -> CvTerm
+-- | fst_congr : CvTerm -> CvTerm
+-- | fst_erased : CvTerm -> CvTerm
+-- | snd_congr : CvTerm -> CvTerm
+-- | snd_erased : CvTerm -> CvTerm
+-- | phi_congr : CvTerm -> CvTerm -> CvTerm -> CvTerm
+-- | phi_erased : CvTerm -> CvTerm
+-- | eq_congr : CvTerm -> CvTerm -> CvTerm -> CvTerm
+-- | refl_congr : CvTerm -> CvTerm
+-- | refl_erased : CvTerm -> CvTerm
+-- | subst_congr : CvTerm -> CvTerm -> CvTerm
+-- | subst_erased : CvTerm -> CvTerm
+-- | conv_congr : CvTerm -> CvTerm -> CvTerm
+-- | conv_erased : CvTerm -> CvTerm
+-- deriving BEq
 
 inductive Term : Type where
 | bound : Const -> Nat -> Term
@@ -76,7 +76,7 @@ inductive Term : Type where
 | lam : Mode -> Term -> Term -> Term
 | app : Mode -> Term -> Term -> Term
 | all : Mode -> Term -> Term -> Term
-| pair : Term -> Term -> Term -> Term
+| pair : Nat -> Term -> Term -> Term -> Term
 | fst : Term -> Term
 | snd : Term -> Term
 | prod : Term -> Term -> Term
@@ -84,7 +84,7 @@ inductive Term : Type where
 | subst : Term -> Term -> Term
 | phi : Term -> Term -> Term -> Term
 | eq : Term -> Term -> Term -> Term
-| conv : Term -> Term -> Nat -> Term
+| conv : Nat -> Term -> Term -> Term
 
 @[reducible]
 def beqfn : Term -> Term -> Bool
@@ -94,7 +94,7 @@ def beqfn : Term -> Term -> Bool
 | .lam m1 x1 x2, .lam m2 y1 y2 => m1 == m2 && beqfn x1 y1 && beqfn x2 y2
 | .app m1 x1 x2, .app m2 y1 y2 => m1 == m2 && beqfn x1 y1 && beqfn x2 y2
 | .all m1 x1 x2, .all m2 y1 y2 => m1 == m2 && beqfn x1 y1 && beqfn x2 y2
-| .pair x1 x2 x3, .pair y1 y2 y3 => beqfn x1 y1 && beqfn x2 y2 && beqfn x3 y3
+| .pair n1 x1 x2 x3, .pair n2 y1 y2 y3 => n1 == n2 && beqfn x1 y1 && beqfn x2 y2 && beqfn x3 y3
 | .fst x1, .fst y1 => beqfn x1 y1
 | .snd x1, .snd y1 => beqfn x1 y1
 | .prod x1 x2, .prod y1 y2 => beqfn x1 y1 && beqfn x2 y2
@@ -102,7 +102,7 @@ def beqfn : Term -> Term -> Bool
 | .subst x1 x2, .subst y1 y2 => beqfn x1 y1 && beqfn x2 y2
 | .phi x1 x2 x3, .phi y1 y2 y3 => beqfn x1 y1 && beqfn x2 y2 && beqfn x3 y3
 | .eq x1 x2 x3, .eq y1 y2 y3 => beqfn x1 y1 && beqfn x2 y2 && beqfn x3 y3
-| .conv x1 x2 n1, .conv y1 y2 n2 => beqfn x1 y1 && beqfn x2 y2 && n1 == n2
+| .conv n1 x1 x2, .conv n2 y1 y2 => n1 == n2 && beqfn x1 y1 && beqfn x2 y2
 | _, _ => false
 
 namespace Term
@@ -116,7 +116,7 @@ namespace Term
   case lam ih1 ih2 _ _ _ => rw [@LawfulBEq.eq_of_beq Mode _ _ _ _ h.1.1, ih1 h.1.2, ih2 h.2]; simp
   case app ih1 ih2 _ _ _ => rw [@LawfulBEq.eq_of_beq Mode _ _ _ _ h.1.1, ih1 h.1.2, ih2 h.2]; simp
   case all ih1 ih2 _ _ _ => rw [@LawfulBEq.eq_of_beq Mode _ _ _ _ h.1.1, ih1 h.1.2, ih2 h.2]; simp
-  case pair ih1 ih2 ih3 _ _ _ => rw [ih1 h.1.1, ih2 h.1.2, ih3 h.2]; simp
+  case pair ih1 ih2 ih3 _ _ _ _ => rw [ih1 h.1.1.2, ih2 h.1.2, ih3 h.2, h.1.1.1]; simp
   case fst ih _ => rw [ih h]
   case snd ih _ => rw [ih h]
   case prod ih1 ih2 _ _ => rw [ih1 h.1, ih2 h.2]; simp
@@ -124,7 +124,7 @@ namespace Term
   case subst ih1 ih2 _ _ => rw [ih1 h.1, ih2 h.2]; simp
   case phi ih1 ih2 ih3 _ _ _ => rw [ih1 h.1.1, ih2 h.1.2, ih3 h.2]; simp
   case eq ih1 ih2 ih3 _ _ _ => rw [ih1 h.1.1, ih2 h.1.2, ih3 h.2]; simp
-  case conv ih1 ih2 _ _ _ => rw [ih1 h.1.1, ih2 h.1.2, h.2]; simp
+  case conv ih1 ih2 _ _ _ => rw [h.1.1, ih1 h.1.2, ih2 h.2]; simp
 
   theorem beq_rfl : {t : Term} -> beqfn t t = true := by
   intro t; induction t <;> simp at * <;> simp [*]
@@ -139,65 +139,68 @@ instance Term_inst_LawfulBEq : LawfulBEq Term where
   eq_of_beq := Term.eq_of_beq
   rfl := Term.beq_rfl
 
+infixl:15 "`@f" => Term.app mf
+infixl:15 "`@τ" => Term.app mt
+infixl:15 "`@0" => Term.app m0
 notation "★" => Term.const Const.type
 notation "□" => Term.const Const.kind
 
 instance instInhabitedTerm : Inhabited Term where
   default := Term.none
 
-namespace CvTerm
+-- namespace CvTerm
 
-  @[simp]
-  def refl : Term -> CvTerm
-  | .bound _ k => .bound k
-  | .none => .none
-  | .const _ => .const
-  | .lam _ t1 t2 => .lam_congr (refl t1) (refl t2)
-  | .app _ t1 t2 => .app_congr (refl t1) (refl t2)
-  | .all _ t1 t2 => .all_congr (refl t1) (refl t2)
-  | .pair t1 t2 t3 => .pair_congr (refl t1) (refl t2) (refl t3)
-  | .fst t => .fst_congr (refl t)
-  | .snd t => .snd_congr (refl t)
-  | .prod t1 t2 => .prod_congr (refl t1) (refl t2)
-  | .refl t => .refl_congr (refl t)
-  | .subst t1 t2 => .subst_congr (refl t1) (refl t2)
-  | .phi t1 t2 t3 => .phi_congr (refl t1) (refl t2) (refl t3)
-  | .eq t1 t2 t3 => .eq_congr (refl t1) (refl t2) (refl t3)
-  | .conv t1 t2 _ => .conv_congr (refl t1) (refl t2)
+--   @[simp]
+--   def refl : Term -> CvTerm
+--   | .bound _ k => .bound k
+--   | .none => .none
+--   | .const _ => .const
+--   | .lam _ t1 t2 => .lam_congr (refl t1) (refl t2)
+--   | .app _ t1 t2 => .app_congr (refl t1) (refl t2)
+--   | .all _ t1 t2 => .all_congr (refl t1) (refl t2)
+--   | .pair t1 t2 t3 => .pair_congr (refl t1) (refl t2) (refl t3)
+--   | .fst t => .fst_congr (refl t)
+--   | .snd t => .snd_congr (refl t)
+--   | .prod t1 t2 => .prod_congr (refl t1) (refl t2)
+--   | .refl t => .refl_congr (refl t)
+--   | .subst t1 t2 => .subst_congr (refl t1) (refl t2)
+--   | .phi t1 t2 t3 => .phi_congr (refl t1) (refl t2) (refl t3)
+--   | .eq t1 t2 t3 => .eq_congr (refl t1) (refl t2) (refl t3)
+--   | .conv t1 t2 _ => .conv_congr (refl t1) (refl t2)
 
-  @[simp]
-  def size : CvTerm -> Nat
-  | .sym c => size c + 1
-  | .trans c1 c2 => size c1 + size c2 + 1
-  | .none => 0
-  | .const => 0
-  | .bound _ => 0
-  | .all_congr c1 c2 => size c1 + size c2 + 1
-  | .lam_congr c1 c2 => size c1 + size c2 + 1
-  | .lam_eta c => size c + 1
-  | .lam_mf_erased c => size c + 1
-  | .lam_m0_erased c => size c + 1
-  | .app_congr c1 c2 => size c1 + size c2 + 1
-  | .app_beta c => size c + 1
-  | .app_m0_erased c => size c + 1
-  | .prod_congr c1 c2 => size c1 + size c2 + 1
-  | .pair_congr c1 c2 c3 => size c1 + size c2 + size c3 + 1
-  | .pair_erased c => size c + 1
-  | .fst_congr c => size c + 1
-  | .fst_erased c => size c + 1
-  | .snd_congr c => size c + 1
-  | .snd_erased c => size c + 1
-  | .phi_congr c1 c2 c3 => size c1 + size c2 + size c3 + 1
-  | .phi_erased c => size c + 1
-  | .eq_congr c1 c2 c3 => size c1 + size c2 + size c3 + 1
-  | .refl_congr c => size c + 1
-  | .refl_erased c => size c + 1
-  | .subst_congr c1 c2 => size c1 + size c2 + 1
-  | .subst_erased c => size c + 1
-  | .conv_congr c1 c2 => size c1 + size c2 + 1
-  | .conv_erased c => size c + 1
+--   @[simp]
+--   def size : CvTerm -> Nat
+--   | .sym c => size c + 1
+--   | .trans c1 c2 => size c1 + size c2 + 1
+--   | .none => 0
+--   | .const => 0
+--   | .bound _ => 0
+--   | .all_congr c1 c2 => size c1 + size c2 + 1
+--   | .lam_congr c1 c2 => size c1 + size c2 + 1
+--   | .lam_eta c => size c + 1
+--   | .lam_mf_erased c => size c + 1
+--   | .lam_m0_erased c => size c + 1
+--   | .app_congr c1 c2 => size c1 + size c2 + 1
+--   | .app_beta c => size c + 1
+--   | .app_m0_erased c => size c + 1
+--   | .prod_congr c1 c2 => size c1 + size c2 + 1
+--   | .pair_congr c1 c2 c3 => size c1 + size c2 + size c3 + 1
+--   | .pair_erased c => size c + 1
+--   | .fst_congr c => size c + 1
+--   | .fst_erased c => size c + 1
+--   | .snd_congr c => size c + 1
+--   | .snd_erased c => size c + 1
+--   | .phi_congr c1 c2 c3 => size c1 + size c2 + size c3 + 1
+--   | .phi_erased c => size c + 1
+--   | .eq_congr c1 c2 c3 => size c1 + size c2 + size c3 + 1
+--   | .refl_congr c => size c + 1
+--   | .refl_erased c => size c + 1
+--   | .subst_congr c1 c2 => size c1 + size c2 + 1
+--   | .subst_erased c => size c + 1
+--   | .conv_congr c1 c2 => size c1 + size c2 + 1
+--   | .conv_erased c => size c + 1
 
-end CvTerm
+-- end CvTerm
 
 namespace Term
 
@@ -209,7 +212,7 @@ namespace Term
   | lam _ t1 t2 => size t1 + size t2 + 1
   | app _ t1 t2 => size t1 + size t2 + 1
   | all _ t1 t2 => size t1 + size t2 + 1
-  | pair t1 t2 t3 => size t1 + size t2 + size t3 + 1
+  | pair _ t1 t2 t3 => size t1 + size t2 + size t3 + 1
   | fst t => size t + 1
   | snd t => size t + 1
   | prod t1 t2 => size t1 + size t2 + 1
@@ -217,34 +220,34 @@ namespace Term
   | subst t1 t2 => size t1 + size t2 + 1
   | phi t1 t2 t3 => size t1 + size t2 + size t3 + 1
   | eq t1 t2 t3 => size t1 + size t2 + size t3 + 1
-  | conv t1 t2 _ => size t1 + size t2 + 1
+  | conv _ t1 t2 => size t1 + size t2 + 1
 
-  inductive IsFreeVar : Nat -> Term -> Prop where
-  | bound : IsFreeVar n (.bound K n)
-  | lam1 : IsFreeVar n A -> IsFreeVar n (.lam m A t)
-  | lam2 : IsFreeVar (n + 1) t -> IsFreeVar n (.lam m A t)
-  | app1 : IsFreeVar n f -> IsFreeVar n (.app m f a)
-  | app2 : IsFreeVar n a -> IsFreeVar n (.app m f a)
-  | all1 : IsFreeVar n A -> IsFreeVar n (.all m A t)
-  | all2 : IsFreeVar (n + 1) t -> IsFreeVar n (.all m A t)
-  | pair1 : IsFreeVar n B -> IsFreeVar n (.pair B t s)
-  | pair2 : IsFreeVar n t -> IsFreeVar n (.pair B t s)
-  | pair3 : IsFreeVar n s -> IsFreeVar n (.pair B t s)
-  | fst : IsFreeVar n t -> IsFreeVar n (.fst t)
-  | snd : IsFreeVar n t -> IsFreeVar n (.snd t)
-  | prod1 : IsFreeVar n A -> IsFreeVar n (.prod A B)
-  | prod2 : IsFreeVar (n + 1) B -> IsFreeVar n (.prod A B)
-  | refl : IsFreeVar n t -> IsFreeVar n (.refl t)
-  | subst1 : IsFreeVar n P -> IsFreeVar n (.subst P e)
-  | subst2 : IsFreeVar n e -> IsFreeVar n (.subst P e)
-  | phi1 : IsFreeVar n a -> IsFreeVar n (.phi a b e)
-  | phi2 : IsFreeVar n b -> IsFreeVar n (.phi a b e)
-  | phi3 : IsFreeVar n e -> IsFreeVar n (.phi a b e)
-  | eq1 : IsFreeVar n A -> IsFreeVar n (.eq A a b)
-  | eq2 : IsFreeVar n a -> IsFreeVar n (.eq A a b)
-  | eq3 : IsFreeVar n b -> IsFreeVar n (.eq A a b)
-  | conv1 : IsFreeVar n B -> IsFreeVar n (.conv B t c)
-  | conv2 : IsFreeVar n t -> IsFreeVar n (.conv B t c)
+  -- inductive IsFreeVar : Nat -> Term -> Prop where
+  -- | bound : IsFreeVar n (.bound K n)
+  -- | lam1 : IsFreeVar n A -> IsFreeVar n (.lam m A t)
+  -- | lam2 : IsFreeVar (n + 1) t -> IsFreeVar n (.lam m A t)
+  -- | app1 : IsFreeVar n f -> IsFreeVar n (.app m f a)
+  -- | app2 : IsFreeVar n a -> IsFreeVar n (.app m f a)
+  -- | all1 : IsFreeVar n A -> IsFreeVar n (.all m A t)
+  -- | all2 : IsFreeVar (n + 1) t -> IsFreeVar n (.all m A t)
+  -- | pair1 : IsFreeVar n B -> IsFreeVar n (.pair B t s)
+  -- | pair2 : IsFreeVar n t -> IsFreeVar n (.pair B t s)
+  -- | pair3 : IsFreeVar n s -> IsFreeVar n (.pair B t s)
+  -- | fst : IsFreeVar n t -> IsFreeVar n (.fst t)
+  -- | snd : IsFreeVar n t -> IsFreeVar n (.snd t)
+  -- | prod1 : IsFreeVar n A -> IsFreeVar n (.prod A B)
+  -- | prod2 : IsFreeVar (n + 1) B -> IsFreeVar n (.prod A B)
+  -- | refl : IsFreeVar n t -> IsFreeVar n (.refl t)
+  -- | subst1 : IsFreeVar n P -> IsFreeVar n (.subst P e)
+  -- | subst2 : IsFreeVar n e -> IsFreeVar n (.subst P e)
+  -- | phi1 : IsFreeVar n a -> IsFreeVar n (.phi a b e)
+  -- | phi2 : IsFreeVar n b -> IsFreeVar n (.phi a b e)
+  -- | phi3 : IsFreeVar n e -> IsFreeVar n (.phi a b e)
+  -- | eq1 : IsFreeVar n A -> IsFreeVar n (.eq A a b)
+  -- | eq2 : IsFreeVar n a -> IsFreeVar n (.eq A a b)
+  -- | eq3 : IsFreeVar n b -> IsFreeVar n (.eq A a b)
+  -- | conv1 : IsFreeVar n B -> IsFreeVar n (.conv B t c)
+  -- | conv2 : IsFreeVar n t -> IsFreeVar n (.conv B t c)
 
 end Term
 
