Common/Term/Normal.lean
@@ -1,33 +1,87 @@
 
 import Common.Term
+import Common.Term.Reduction
 
 namespace Term
 
-  mutual
-    inductive Neutral : Term -> Prop where
-    | bound : Neutral (.bound c k)
-    | app : Neutral f ->  Normal a -> Neutral (.app m f a)
-    | fst : Neutral t -> Neutral (.fst t)
-    | snd : Neutral t -> Neutral (.snd t)
-    | subst : Normal P -> Neutral e -> Neutral (.subst P e)
-    | phi :  Normal a ->  Normal b -> Neutral e -> Neutral (.phi a b e)
-    | conv :  Normal B ->  Neutral t -> Neutral (.conv B t c)
+  def Reducible (t : Term) := ∃ t', t -β> t'
+  def Normal (t : Term) := ¬ (Reducible t)
+  abbrev NormalForm (t : Term) (t' : Term) := t -β>* t' ∧ Normal t'
+  def WN (t : Term) := ∃ t', NormalForm t t'
 
-    inductive Normal : Term -> Prop where
-    | bound : Normal (.bound c k)
-    | const : Normal (.const K)
-    | lam : Normal A -> Normal t -> Normal (.lam m A t)
-    | app : Neutral f -> Normal a -> Normal (.app m f a)
-    | all : Normal A -> Normal B -> Normal (.all m A B)
-    | pair : Normal T -> Normal t -> Normal s -> Normal (.pair T t s)
-    | fst : Neutral t -> Normal (.fst t)
-    | snd : Neutral t -> Normal (.snd t)
-    | prod : Normal A -> Normal B -> Normal (.prod A B)
-    | refl : Normal t -> Normal (.refl t)
-    | subst : Normal P -> Neutral e -> Normal (.subst P e)
-    | phi : Normal a -> Normal b -> Neutral e -> Normal (.phi a b e)
-    | eq : Normal A -> Normal a -> Normal b -> Normal (.eq A a b)
-    | conv : Normal B -> Normal t -> Normal (.conv B t c)
-  end
+  inductive SN : Term -> Prop where
+  | sn : (∀ y, x -β> y -> SN y) -> SN x
+
+  theorem sn_preimage (f : Term -> Term) x : (∀ x y, x -β> y -> (f x) -β> (f y)) -> SN (f x) -> SN x := by
+  intro h sh
+  generalize zdef : f x = z at sh
+  induction sh generalizing f x
+  case _ x' h' ih =>
+    subst zdef; constructor
+    intro y r
+    apply ih (f y) (h _ _ r) f y h rfl
+
+  theorem sn_closed : SN (.app m f a) -> SN f := by
+  apply sn_preimage (λ f => .app m f a);
+  intro f f'; apply Red.app_congr1
+
+  theorem sn_subst : SN ([σ]t) -> SN t := by
+  apply sn_preimage (Subst.apply σ)
+  intro x y r; apply Red.subst1_same σ r
+
+  theorem sn_implies_wn : SN t -> WN t := by
+  intro h
+  induction h
+  case sn t' _ ih =>
+    have lem : Reducible t' ∨ Normal t' := by apply Classical.em
+    cases lem
+    case _ h' =>
+      cases h'
+      case _ t'' h' =>
+        have lem := ih _ h'
+        cases lem
+        case _ z lem =>
+          exists z; apply And.intro
+          apply Term.RedStar.step; apply h'; apply lem.1
+          apply lem.2
+    case _ h' =>
+      exists t'; apply And.intro; apply Term.Red.refl
+      apply h'
+
+  -- theorem normal_lam : Normal (.lam m A t) -> Normal A ∧ Normal t := by sorry
+  -- theorem normal_app : Normal (.app m f a) -> Normal f ∧ Normal a ∧ (∀ A t, f ≠ .lam m A t) := by sorry
+  -- theorem normal_all : Normal (.all m A B) -> Normal A ∧ Normal B := by sorry
+  -- theorem normal_pair : Normal (.pair B t s) -> Normal B ∧ Normal t ∧ Normal s := by sorry
+  -- theorem normal_fst : Normal (.fst t) -> Normal t ∧ (∀ B f s, t ≠ .pair B f s) := by sorry
+  -- theorem normal_snd : Normal (.snd t) -> Normal t ∧ (∀ B f s, t ≠ .pair B f s) := by sorry
+  -- theorem normal_prod : Normal (.prod A B) -> Normal A ∧ Normal B := by sorry
+  -- theorem normal_refl : Normal (.refl t) -> Normal t := by sorry
+  -- theorem normal_subst : Normal (.subst Pr e) -> Normal Pr ∧ Normal e ∧ (∀ t, e ≠ refl t) := by sorry
+  -- theorem normal_phi : Normal (.phi a b e) -> Normal a ∧ Normal b ∧ Normal e ∧ (∀ t, e ≠ refl t) := by sorry
+  -- theorem normal_eq : Normal (.eq A a b) -> Normal A ∧ Normal a ∧ Normal b := by sorry
+  -- theorem normal_conv : Normal (.conv B t n) -> Normal B ∧ Normal t := by sorry
+
+  inductive ValueVariant where
+  | nf : ValueVariant
+  | ne : ValueVariant
+
+  inductive Value : ValueVariant -> Term -> Prop where
+  -- Neutral Forms
+  | bound : Value .ne (.bound c k)
+  | app : Value .ne f -> Value .nf a -> Value .ne (.app m f a)
+  | fst : Value .ne t -> Value .ne (.fst t)
+  | snd : Value .ne t -> Value .ne (.snd t)
+  | subst : Value .nf Pr -> Value .ne e -> Value .ne (.subst Pr e)
+  | phi : Value .nf a -> Value .nf b -> Value .ne e -> Value .ne (.phi a b e)
+  -- Normal Forms
+  | const : Value .nf (.const K)
+  | lam : Value .nf A -> Value .nf t -> Value .nf (.lam m A t)
+  | all : Value .nf A -> Value .nf B -> Value .nf (.all m A B)
+  | pair : Value .nf T -> Value .nf t -> Value .nf s -> Value .nf (.pair n T t s)
+  | prod : Value .nf A -> Value .nf B -> Value .nf (.prod A B)
+  | refl : Value .nf t -> Value .nf (.refl t)
+  | eq : Value .nf A -> Value .nf a -> Value .nf b -> Value .nf (.eq A a b)
+  | conv : Value .nf B -> Value .nf t -> Value .nf (.conv n B t)
+  | neutral : Value .ne t -> Value .nf t
 
 end Term
