Common/Term/Reduction.lean
@@ -4,25 +4,48 @@ import Common.Term.Substitution
 namespace Term
 
   inductive Red : Term -> Term -> Prop where
+  -- Basic reduction Steps
   | beta : Red (.app m (.lam m A b) t) (b β[t])
-  | proj1 : Red (.fst (.pair B t s)) t
-  | proj2 : Red (.snd (.pair B t s)) s
-  | substelim : Red (.subst B (.refl t)) (.lam mf (.app mt B t) (.bound .type 0))
-  | conv_lam : Red (.conv (.all m A1 B) (.lam m A2 t) n) (.lam m A2 (.conv B t n))
-  | conv_pair : Red (.conv T (.pair T t s) n) (.pair T t s)
-  | conv_refl : Red (.conv (.eq A t t) (.refl t) n) (.refl (conv A t n))
-  | conv_all : Red (.conv (.const K) (.all m A B) n) (.all m A B)
-  | conv_prod : Red (.conv ★ (.prod A B) n) (.prod A B)
-  | conv_eq : Red (.conv ★ (.eq A a b) n) (.eq A a b)
+  | proj1 : Red (.fst (.pair n B t s)) t
+  | proj2 : Red (.snd (.pair n B t s)) s
+  | substelim : Red (.subst Pr (.refl t)) (.lam mf (Pr `@τ t `@τ .refl t) (.bound .type 0))
+  | phi : Red (.phi a b (.refl t)) b
+  -- Weak conversion passthrough reduction steps
+  -- .app m (.conv n (.all m A1 B1) (.all m A2 B2) b) t -β>
+  --   .conv n (B1 β[t]) (B2 β[.conv n A2 t]) (.app m b (.conv n A2 t))
+
+  -- .fst (.conv n (.prod A1 B1) (.prod A2 B2) t) -β>
+  --   .conv n A1 A2 (.fst t)
+
+  -- .snd (.conv n (.prod A1 B1) (.prod A2 B2) t) -β>
+  --   .conv n (B1 β[.conv n A1 (.fst t)]) (B2 β[.fst t]) (.snd t)
+
+  -- .subst Pr (.conv n (.eq A1 a1 b1) (.eq A2 a2 b2) t) -β>
+  --   .conv n (Pr a1 (.refl a1) -> Pr b1 (.conv n (.eq A1 a1 b1) (.eq A2 a2 b2) t))
+  --           (Pr a2 (.refl a2) -> Pr b2 t)
+  --     (.subst Pr t)
+
+  -- .phi B a' b' (.conv n (.eq A1 a1 b1) (.eq A2 a2 b2) t) -β>
+  --   .conv n (.prod A1 B) (.prod A2 B) (.phi a' b' t)
+  | conv_beta : Red (.app m (.conv n (.all m A1 B) (.lam m A2 b)) t) (.conv n (B β[t]) (b β[.conv n A2 t]))
+  | conv_fst : Red (.fst (.conv n (.prod A B1) (.pair n2 B2 t s))) (.conv n A t)
+  | conv_snd : Red (.snd (.conv n (.prod A B1) (.pair n2 B2 t s))) (.conv n (B1 β[.conv n A t]) s)
+  | conv_subst :
+    Red (.subst Pr (.conv n (.eq A a b) (.refl t)))
+      (.conv n (.all mf (Pr `@τ a `@τ .refl a) (Pr `@τ b `@τ (.conv n (.eq A a b) (.refl t))))
+        (.lam mf (Pr `@τ t `@τ .refl t) (.bound .type 0)))
+  | conv_phi : Red (.phi a b (.conv n (.eq A x y) (.refl t))) b
+  | conv_conv : Red (.conv n1 A (.conv n2 B t)) (.conv (n1 + n2) A t)
+  -- Congruences
   | lam_congr1 : Red A A' -> Red (.lam m A t) (.lam m A' t)
   | lam_congr2 : Red t t' -> Red (.lam m A t) (.lam m A t')
   | app_congr1 : Red f f' -> Red (.app m f t) (.app m f' t)
   | app_congr2 : Red t t' -> Red (.app m f t) (.app m f t')
   | all_congr1 : Red A A' -> Red (.all m A B) (.all m A' B)
   | all_congr2 : Red B B' -> Red (.all m A B) (.all m A B')
-  | pair_congr1 : Red B B' -> Red (.pair B t s) (.pair B' t s)
-  | pair_congr2 : Red t t' -> Red (.pair B t s) (.pair B t' s)
-  | pair_congr3 : Red s s' -> Red (.pair B t s) (.pair B t s')
+  | pair_congr1 : Red B B' -> Red (.pair n B t s) (.pair n B' t s)
+  | pair_congr2 : Red t t' -> Red (.pair n B t s) (.pair n B t' s)
+  | pair_congr3 : Red s s' -> Red (.pair n B t s) (.pair n B t s')
   | fst_congr : Red t t' -> Red (.fst t) (.fst t')
   | snd_congr : Red t t' -> Red (.snd t) (.snd t')
   | prod_congr1 : Red A A' -> Red (.prod A B) (.prod A' B)
@@ -36,93 +59,101 @@ namespace Term
   | eq_congr1 : Red A A' -> Red (.eq A a b) (.eq A' a b)
   | eq_congr2 : Red a a' -> Red (.eq A a b) (.eq A a' b)
   | eq_congr3 : Red b b' -> Red (.eq A a b) (.eq A a b')
-  | conv_congr1 : Red A A' -> Red (.conv A t n) (.conv A' t n)
-  | conv_congr2 : Red t t' -> Red (.conv A t n) (.conv A t' n)
+  | conv_congr1 : Red A A' -> Red (.conv n A t) (.conv n A' t)
+  | conv_congr2 : Red t t' -> Red (.conv n A t) (.conv n A t')
 
   inductive RedStar : Term -> Term -> Prop where
   | refl : RedStar t t
   | step : Red x y -> RedStar y z -> RedStar x z
 
+  inductive RedBounded : Nat -> Term -> Term -> Prop where
+  | refl : RedBounded n t t
+  | step : Red x y -> RedBounded n y z -> RedBounded (n + 1) x z
+
   abbrev RedConv (A : Term) (B : Term) : Prop := ∃ C, RedStar A C ∧ RedStar B C
 
-  inductive ParRed : Term -> Term -> Prop where
-  | bound : ParRed (.bound K n) (.bound K n)
-  | none : ParRed .none .none
-  | const : ParRed (.const K) (.const K)
-  | beta : ParRed A A' -> ParRed b b' -> ParRed t t' -> ParRed (.app m (.lam m A b) t) (b' β[t'])
-  | proj1 : ParRed B B' -> ParRed t t' -> ParRed s s' -> ParRed (.fst (.pair B t s)) t'
-  | proj2 : ParRed B B' -> ParRed t t' -> ParRed s s' -> ParRed (.snd (.pair B t s)) s'
-  | substelim : ParRed B B' -> ParRed t t' -> ParRed (.subst B (.refl t)) (.lam mf (.app mt B' t') (.bound .type 0))
-  | conv_lam : ParRed B B' -> ParRed A2 A2' -> ParRed t t' ->
-    ParRed (.conv (.all m A1 B) (.lam m A2 t) n) (.lam m A2' (.conv B' t' n))
-  | conv_pair : ParRed T T' -> ParRed t t' -> ParRed s s' ->
-    ParRed (.conv T (.pair T t s) n) (.pair T' t' s')
-  | conv_refl : ParRed A A' -> ParRed t t' ->
-    ParRed (.conv (.eq A t t) (.refl t) n) (.refl (conv A' t' n))
-  | conv_all : ParRed A A' -> ParRed B B' ->
-    ParRed (.conv (.const K) (.all m A B) n) (.all m A' B')
-  | conv_prod : ParRed A A' -> ParRed B B' ->
-    ParRed (.conv ★ (.prod A B) n) (.prod A' B')
-  | conv_eq : ParRed A A' -> ParRed a a' -> ParRed b b' ->
-    ParRed (.conv ★ (.eq A a b) n) (.eq A' a' b')
-  | lam_congr : ParRed A A' -> ParRed t t' -> ParRed (.lam m A t) (.lam m A' t')
-  | app_congr : ParRed f f' -> ParRed a a' -> ParRed (.app m f a) (.app m f' a')
-  | all_congr : ParRed A A' -> ParRed B B' -> ParRed (.all m A B) (.all m A' B')
-  | pair_congr : ParRed B B' -> ParRed t t' -> ParRed s s' -> ParRed (.pair B t s) (.pair B' t' s')
-  | fst_congr : ParRed t t' -> ParRed (.fst t) (.fst t')
-  | snd_congr : ParRed t t' -> ParRed (.snd t) (.snd t')
-  | prod_congr : ParRed A A' -> ParRed B B' -> ParRed (.prod A B) (.prod A' B')
-  | refl_congr : ParRed t t' -> ParRed (.refl t) (.refl t')
-  | subst_congr : ParRed B B' -> ParRed e e' -> ParRed (.subst B e) (.subst B' e')
-  | phi_congr : ParRed a a' -> ParRed b b' -> ParRed e e' -> ParRed (.phi a b e) (.phi a' b' e')
-  | eq_congr : ParRed A A' -> ParRed a a' -> ParRed b b' -> ParRed (.eq A a b) (.eq A' a' b')
-  | conv_congr : ParRed A A' -> ParRed t t' -> ParRed (.conv A t c) (.conv A' t' c)
+  abbrev RedConvBounded (n : Nat) (A : Term) (B : Term) : Prop := ∃ C, RedBounded n A C ∧ RedBounded n B C
 
-  @[simp]
-  def pcompl : Term -> Term
-  | .app mf (.lam mf _ b) t
-  | .app m0 (.lam m0 _ b) t
-  | .app mt (.lam mt _ b) t => (pcompl b) β[pcompl t]
-  | .fst (.pair _ t _) => pcompl t
-  | .snd (.pair _ _ s) => pcompl s
-  | .subst B (.refl t) => .lam mf (.app mt (pcompl B) (pcompl t)) (.bound .type 0)
-  | .conv (.all m1 A1 B) (.lam m2 A2 t) n => .lam m2 (pcompl A2) (.conv (pcompl B) (pcompl t) n)
-  | .conv T1 (.pair T2 t s) n =>
-    if T1 == T2 then .pair (pcompl T1) (pcompl t) (pcompl s)
-    else .conv (pcompl T1) (pcompl (.pair T2 t s)) n
-  | .conv (.eq A t1 t2) (.refl t3) n =>
-    if t1 == t2 && t2 == t3 then .refl (conv (pcompl A) (pcompl t1) n)
-    else .conv (pcompl (.eq A t1 t2)) (pcompl (.refl t3)) n
-  | .conv (.const _) (.all m A B) _ => .all m (pcompl A) (pcompl B)
-  | .conv ★ (.prod A B) _ => .prod (pcompl A) (pcompl B)
-  | .conv ★ (.eq A a b) _ => .eq (pcompl A) (pcompl a) (pcompl b)
-  | .lam m A t => .lam m (pcompl A) (pcompl t)
-  | .app m f a => .app m (pcompl f) (pcompl a)
-  | .all m A B => .all m (pcompl A) (pcompl B)
-  | .pair B t s => .pair (pcompl B) (pcompl t) (pcompl s)
-  | .fst t => .fst (pcompl t)
-  | .snd t => .snd (pcompl t)
-  | .prod A B => .prod (pcompl A) (pcompl B)
-  | .refl t => .refl (pcompl t)
-  | .subst B e => .subst (pcompl B) (pcompl e)
-  | .phi a b e => .phi (pcompl a) (pcompl b) (pcompl e)
-  | .eq A a b => .eq (pcompl A) (pcompl a) (pcompl b)
-  | .conv A t c => .conv (pcompl A) (pcompl t) c
-  | .bound K n => .bound K n
-  | .const K => .const K
-  | .none => .none
+  -- inductive ParRed : Term -> Term -> Prop where
+  -- | bound : ParRed (.bound K n) (.bound K n)
+  -- | none : ParRed .none .none
+  -- | const : ParRed (.const K) (.const K)
+  -- | beta : ParRed A A' -> ParRed b b' -> ParRed t t' -> ParRed (.app m (.lam m A b) t) (b' β[t'])
+  -- | proj1 : ParRed B B' -> ParRed t t' -> ParRed s s' -> ParRed (.fst (.pair B t s)) t'
+  -- | proj2 : ParRed B B' -> ParRed t t' -> ParRed s s' -> ParRed (.snd (.pair B t s)) s'
+  -- | substelim : ParRed B B' -> ParRed t t' -> ParRed (.subst B (.refl t)) (.lam mf (.app mt B' t') (.bound .type 0))
+  -- | conv_lam : ParRed B B' -> ParRed A2 A2' -> ParRed t t' ->
+  --   ParRed (.conv (.all m A1 B) (.lam m A2 t) n) (.lam m A2' (.conv B' t' n))
+  -- | conv_pair : ParRed T T' -> ParRed t t' -> ParRed s s' ->
+  --   ParRed (.conv T (.pair T t s) n) (.pair T' t' s')
+  -- | conv_refl : ParRed A A' -> ParRed t t' ->
+  --   ParRed (.conv (.eq A t t) (.refl t) n) (.refl (conv A' t' n))
+  -- | conv_all : ParRed A A' -> ParRed B B' ->
+  --   ParRed (.conv (.const K) (.all m A B) n) (.all m A' B')
+  -- | conv_prod : ParRed A A' -> ParRed B B' ->
+  --   ParRed (.conv ★ (.prod A B) n) (.prod A' B')
+  -- | conv_eq : ParRed A A' -> ParRed a a' -> ParRed b b' ->
+  --   ParRed (.conv ★ (.eq A a b) n) (.eq A' a' b')
+  -- | lam_congr : ParRed A A' -> ParRed t t' -> ParRed (.lam m A t) (.lam m A' t')
+  -- | app_congr : ParRed f f' -> ParRed a a' -> ParRed (.app m f a) (.app m f' a')
+  -- | all_congr : ParRed A A' -> ParRed B B' -> ParRed (.all m A B) (.all m A' B')
+  -- | pair_congr : ParRed B B' -> ParRed t t' -> ParRed s s' -> ParRed (.pair B t s) (.pair B' t' s')
+  -- | fst_congr : ParRed t t' -> ParRed (.fst t) (.fst t')
+  -- | snd_congr : ParRed t t' -> ParRed (.snd t) (.snd t')
+  -- | prod_congr : ParRed A A' -> ParRed B B' -> ParRed (.prod A B) (.prod A' B')
+  -- | refl_congr : ParRed t t' -> ParRed (.refl t) (.refl t')
+  -- | subst_congr : ParRed B B' -> ParRed e e' -> ParRed (.subst B e) (.subst B' e')
+  -- | phi_congr : ParRed a a' -> ParRed b b' -> ParRed e e' -> ParRed (.phi a b e) (.phi a' b' e')
+  -- | eq_congr : ParRed A A' -> ParRed a a' -> ParRed b b' -> ParRed (.eq A a b) (.eq A' a' b')
+  -- | conv_congr : ParRed A A' -> ParRed t t' -> ParRed (.conv A t c) (.conv A' t' c)
 
-  inductive ParRedStar : Term -> Term -> Prop where
-  | refl : ParRedStar t t
-  | step : ParRed x y -> ParRedStar y z -> ParRedStar x z
+  -- @[simp]
+  -- def pcompl : Term -> Term
+  -- | .app mf (.lam mf _ b) t
+  -- | .app m0 (.lam m0 _ b) t
+  -- | .app mt (.lam mt _ b) t => (pcompl b) β[pcompl t]
+  -- | .fst (.pair _ t _) => pcompl t
+  -- | .snd (.pair _ _ s) => pcompl s
+  -- | .subst B (.refl t) => .lam mf (.app mt (pcompl B) (pcompl t)) (.bound .type 0)
+  -- | .conv (.all m1 A1 B) (.lam m2 A2 t) n => .lam m2 (pcompl A2) (.conv (pcompl B) (pcompl t) n)
+  -- | .conv T1 (.pair T2 t s) n =>
+  --   if T1 == T2 then .pair (pcompl T1) (pcompl t) (pcompl s)
+  --   else .conv (pcompl T1) (pcompl (.pair T2 t s)) n
+  -- | .conv (.eq A t1 t2) (.refl t3) n =>
+  --   if t1 == t2 && t2 == t3 then .refl (conv (pcompl A) (pcompl t1) n)
+  --   else .conv (pcompl (.eq A t1 t2)) (pcompl (.refl t3)) n
+  -- | .conv (.const _) (.all m A B) _ => .all m (pcompl A) (pcompl B)
+  -- | .conv ★ (.prod A B) _ => .prod (pcompl A) (pcompl B)
+  -- | .conv ★ (.eq A a b) _ => .eq (pcompl A) (pcompl a) (pcompl b)
+  -- | .lam m A t => .lam m (pcompl A) (pcompl t)
+  -- | .app m f a => .app m (pcompl f) (pcompl a)
+  -- | .all m A B => .all m (pcompl A) (pcompl B)
+  -- | .pair B t s => .pair (pcompl B) (pcompl t) (pcompl s)
+  -- | .fst t => .fst (pcompl t)
+  -- | .snd t => .snd (pcompl t)
+  -- | .prod A B => .prod (pcompl A) (pcompl B)
+  -- | .refl t => .refl (pcompl t)
+  -- | .subst B e => .subst (pcompl B) (pcompl e)
+  -- | .phi a b e => .phi (pcompl a) (pcompl b) (pcompl e)
+  -- | .eq A a b => .eq (pcompl A) (pcompl a) (pcompl b)
+  -- | .conv A t c => .conv (pcompl A) (pcompl t) c
+  -- | .bound K n => .bound K n
+  -- | .const K => .const K
+  -- | .none => .none
 
-  abbrev ParRedConv (A : Term) (B : Term) : Prop := ∃ C, ParRedStar A C ∧ ParRedStar B C
+  -- inductive ParRedStar : Term -> Term -> Prop where
+  -- | refl : ParRedStar t t
+  -- | step : ParRed x y -> ParRedStar y z -> ParRedStar x z
+
+  -- abbrev ParRedConv (A : Term) (B : Term) : Prop := ∃ C, ParRedStar A C ∧ ParRedStar B C
 
 end Term
 
 infix:40 " -β> " => Term.Red
 infix:39 " -β>* " => Term.RedStar
+notation:39 t:39 " -β>{" n "} " s:39 => Term.RedBounded n t s
 infix:38 " =β= " => Term.RedConv
+notation:38 t:38 " =β{" n "}= " s:38 => Term.RedConvBounded n t s
 infix:40 " =β> " => Term.ParRed
 infix:39 " =β>* " => Term.ParRedStar
 infix:38 " ≡β≡ " => Term.ParRedConv
@@ -145,40 +176,41 @@ namespace Red
   case _ => simp [*]
   case _ h2 _h3 ih =>  apply ih (trans_flip h1 h2)
 
-  theorem subst1_same σ : t -β> s -> [σ]t -β> [σ]s := by
-  intro h
-  induction h generalizing σ
-  all_goals try (case _ ih => simp; constructor; apply ih)
-  case beta m A b t =>
-    have h := @Red.beta m ([σ]A) ([^σ]b) ([σ]t)
-    simp at *; exact h
-  case proj1 B t s =>
-    have h := @Red.proj1 ([σ]B) ([σ]t) ([σ]s)
-    simp at *; exact h
-  case proj2 B t s =>
-    have h := @Red.proj2 ([σ]B) ([σ]t) ([σ]s)
-    simp at *; exact h
-  case substelim B t =>
-    have h := @Red.substelim ([σ]B) ([σ]t)
-    simp at *; exact h
-  case conv_lam m A1 B A2 t n =>
-    have h := @Red.conv_lam m ([σ]A1) ([^σ]B) ([σ]A2) ([^σ]t) n
-    simp at *; exact h
-  case conv_pair T t s n =>
-    have h := @Red.conv_pair ([σ]T) ([σ]t) ([σ]s) n
-    simp at *; exact h
-  case conv_refl A t n =>
-    have h := @Red.conv_refl ([σ]A) ([σ]t) n
-    simp at *; exact h
-  case conv_all K m A B n =>
-    have h := @Red.conv_all K m ([σ]A) ([^σ]B) n
-    simp at *; exact h
-  case conv_prod A B n =>
-    have h := @Red.conv_prod ([σ]A) ([^σ]B) n
-    simp at *; exact h
-  case conv_eq A a b n =>
-    have h := @Red.conv_eq ([σ]A) ([σ]a) ([σ]b) n
-    simp at *; exact h
+  theorem subst1_same σ : t -β> s -> [σ]t -β> [σ]s := by sorry
+  -- intro h
+  -- induction h generalizing σ
+  -- all_goals try (case _ ih => simp; constructor; apply ih)
+  -- case beta m A b t =>
+  --   have h := @Red.beta m ([σ]A) ([^σ]b) ([σ]t)
+  --   simp at *; exact h
+  -- case proj1 B t s =>
+  --   have h := @Red.proj1 ([σ]B) ([σ]t) ([σ]s)
+  --   simp at *; exact h
+  -- case proj2 B t s =>
+  --   have h := @Red.proj2 ([σ]B) ([σ]t) ([σ]s)
+  --   simp at *; exact h
+  -- case substelim B t =>
+  --   have h := @Red.substelim ([σ]B) ([σ]t)
+  --   simp at *; exact h
+  -- -- case conv_lam m A1 B A2 t n =>
+  -- --   have h := @Red.conv_lam m ([σ]A1) ([^σ]B) ([σ]A2) ([^σ]t) n
+  -- --   simp at *; exact h
+  -- -- case conv_pair T t s n =>
+  -- --   have h := @Red.conv_pair ([σ]T) ([σ]t) ([σ]s) n
+  -- --   simp at *; exact h
+  -- -- case conv_refl A t n =>
+  -- --   have h := @Red.conv_refl ([σ]A) ([σ]t) n
+  -- --   simp at *; exact h
+  -- case conv_all K m A B n =>
+  --   have h := @Red.conv_all K m ([σ]A) ([^σ]B) n
+  --   simp at *; exact h
+  -- case conv_prod A B n =>
+  --   have h := @Red.conv_prod ([σ]A) ([^σ]B) n
+  --   simp at *; exact h
+  -- case conv_eq A a b n =>
+  --   have h := @Red.conv_eq ([σ]A) ([σ]a) ([σ]b) n
+  --   simp at *; exact h
+  -- repeat sorry
 
   theorem subst_same σ : t -β>* s -> [σ]t -β>* [σ]s := by
   intro h
@@ -373,523 +405,525 @@ namespace Red
 
 end Red
 
-namespace ParRed
+-- namespace ParRed
 
-  @[simp]
-  theorem refl1 t : t =β> t := by
-  induction t; all_goals constructor <;> simp [*]
+--   @[simp]
+--   theorem refl1 t : t =β> t := by
+--   induction t; all_goals constructor <;> simp [*]
 
-  theorem refl t : t =β>* t := by constructor
+--   theorem refl t : t =β>* t := by constructor
 
-  theorem trans_flip : x =β>* y -> y =β> z -> x =β>* z := by
-  intro h1 h2
-  induction h1
-  case _ => apply ParRedStar.step h2; apply refl
-  case _ h3 _h4 ih =>  apply ParRedStar.step h3 (ih h2)
+--   theorem trans_flip : x =β>* y -> y =β> z -> x =β>* z := by
+--   intro h1 h2
+--   induction h1
+--   case _ => apply ParRedStar.step h2; apply refl
+--   case _ h3 _h4 ih =>  apply ParRedStar.step h3 (ih h2)
 
-  theorem trans : x =β>* y -> y =β>* z -> x =β>* z := by
-  intro h1 h2
-  induction h2; simp [*]
-  case _ r1 _r2 ih =>
-    apply ih; apply trans_flip h1 r1
+--   theorem trans : x =β>* y -> y =β>* z -> x =β>* z := by
+--   intro h1 h2
+--   induction h2; simp [*]
+--   case _ r1 _r2 ih =>
+--     apply ih; apply trans_flip h1 r1
 
-  theorem from_red : s -β> t -> s =β> t := by
-  intro h
-  induction h
-  all_goals (try constructor <;> simp [*])
-  case beta => constructor; repeat apply refl1
-  case proj1 => constructor; repeat apply refl1
-  case proj2 => constructor; repeat apply refl1
+--   theorem from_red : s -β> t -> s =β> t := by
+--   intro h
+--   induction h
+--   all_goals (try constructor <;> simp [*])
+--   case beta => constructor; repeat apply refl1
+--   case proj1 => constructor; repeat apply refl1
+--   case proj2 => constructor; repeat apply refl1
+--   repeat sorry
 
-  theorem from_redstar : s -β>* t -> s =β>* t := by
-  intro h
-  induction h
-  case _ => constructor
-  case _ h1 _h2 ih => constructor; apply (from_red h1); apply ih
+--   theorem from_redstar : s -β>* t -> s =β>* t := by
+--   intro h
+--   induction h
+--   case _ => constructor
+--   case _ h1 _h2 ih => constructor; apply (from_red h1); apply ih
 
-  theorem to_red : s =β> t -> s -β>* t := by
-  intro h
-  induction h
-  case bound => apply Term.Red.refl
-  case none => apply Term.Red.refl
-  case const => apply Term.Red.refl
-  case beta A _A' b b' t t' m _ _ _ _ih1 ih2 ih3 =>
-    have r1 := Red.congr2 (λ b t => .app m (.lam m A b) t)
-      (by {
-        intro t1 t2 t1' h; simp
-        apply Red.app_congr1; apply Red.lam_congr2; apply h
-      })
-      (by {
-        intro t1 t2 t2' h; simp
-        apply Red.app_congr2; apply h
-      })
-      ih2 ih3
-    simp at r1
-    apply Red.trans_flip; apply r1; constructor
-  case proj1 B _B' t t' s _s' _ _ _ _ih1 ih2 _ih3 =>
-    have r1 := Red.congr1 (λ t => .fst (.pair B t s))
-      (by {
-        intro t t' h; simp
-        apply Red.fst_congr; apply Red.pair_congr2; apply h
-      })
-      ih2
-    simp at r1
-    apply Red.trans_flip; apply r1; constructor
-  case proj2 B _B' t _t' s s' _ _ _ _ih1 _ih2 ih3 =>
-    have r1 := Red.congr1 (λ s => .snd (.pair B t s))
-      (by {
-        intro t t' h; simp
-        apply Red.snd_congr; apply Red.pair_congr3; apply h
-      })
-      ih3
-    simp at r1
-    apply Red.trans_flip; apply r1; constructor
-  case substelim B B' t t' _ _ ih1 ih2 =>
-    have r1 := Red.congr2 (λ B t => .subst B (.refl t))
-      (by {
-        intro t1 t2 t1' h; simp
-        apply Red.subst_congr1; apply h
-      })
-      (by {
-        intro t1 t2 t2' h; simp
-        apply Red.subst_congr2; apply Red.refl_congr; apply h
-      })
-      ih1 ih2
-    simp at r1
-    apply Red.trans_flip; apply r1; constructor
-  case conv_lam B B' A2 A2' t t' m A1 n _ _ ih1 ih2 ih3 ih4 =>
-    apply Red.trans; apply Red.congr1 (λ A2 => (all m A1 B).conv (lam m A2 t) n)
-    intro t1 t1' h; apply Red.conv_congr2; apply Red.lam_congr1; apply h
-    apply ih3;
-    apply RedStar.step; apply Red.conv_lam
-    apply Red.congr2 (λ B t => lam m A2' (conv B t n))
-    intro t1 t2 t1' h; apply Red.lam_congr2; apply Red.conv_congr1; apply h
-    intro t1 t2 t2' h; apply Red.lam_congr2; apply Red.conv_congr2; apply h
-    apply ih2; apply ih4
-  case conv_pair T T' t t' s s' n _ _ _ ih1 ih2 ih3 =>
-    apply RedStar.step; constructor
-    apply Red.congr3 (λ T t s => pair T t s)
-    intro t1 t2 t3 t1' h; apply Red.pair_congr1; apply h
-    intro t1 t2 t3 t2' h; apply Red.pair_congr2; apply h
-    intro t1 t2 t3 t3' h; apply Red.pair_congr3; apply h
-    apply ih1; apply ih2; apply ih3
-  case conv_refl A A' t t' n _ _ ih1 ih2 =>
-    apply RedStar.step; constructor
-    apply Red.congr2 (λ A t => Term.refl (conv A t n))
-    intro t1 t2 t1' h; apply Red.refl_congr; apply Red.conv_congr1; apply h
-    intro t1 t2 t2' h; apply Red.refl_congr; apply Red.conv_congr2; apply h
-    apply ih1; apply ih2
-  case conv_all A A' B B' K m n _ _ ih1 ih2 =>
-    apply RedStar.step; constructor
-    apply Red.congr2 (λ A B => all m A B)
-    intro t1 t2 t1' h; apply Red.all_congr1; apply h
-    intro t1 t2 t2' h; apply Red.all_congr2; apply h
-    apply ih1; apply ih2
-  case conv_prod A A' B B' n _ _ ih1 ih2 =>
-    apply RedStar.step; constructor
-    apply Red.congr2 (λ A B => prod A B)
-    intro t1 t2 t1' h; apply Red.prod_congr1; apply h
-    intro t1 t2 t2' h; apply Red.prod_congr2; apply h
-    apply ih1; apply ih2
-  case conv_eq A A' a a' b b' n _ _ _ ih1 ih2 ih3 =>
-    apply RedStar.step; constructor
-    apply Red.congr3 (λ A a b => eq A a b)
-    intro t1 t2 t3 t1' h; apply Red.eq_congr1; apply h
-    intro t1 t2 t3 t2' h; apply Red.eq_congr2; apply h
-    intro t1 t2 t3 t3' h; apply Red.eq_congr3; apply h
-    apply ih1; apply ih2; apply ih3
-  case lam_congr ih1 ih2 => apply Red.congr2 (.lam _) .lam_congr1 .lam_congr2 ih1 ih2
-  case app_congr ih1 ih2 => apply Red.congr2 (.app _) .app_congr1 .app_congr2 ih1 ih2
-  case all_congr ih1 ih2 => apply Red.congr2 (.all _) .all_congr1 .all_congr2 ih1 ih2
-  case pair_congr ih1 ih2 ih3 => apply Red.congr3 .pair .pair_congr1 .pair_congr2 .pair_congr3 ih1 ih2 ih3
-  case fst_congr ih => apply Red.congr1 .fst .fst_congr ih
-  case snd_congr ih => apply Red.congr1 .snd .snd_congr ih
-  case prod_congr ih1 ih2 => apply Red.congr2 .prod .prod_congr1 .prod_congr2 ih1 ih2
-  case refl_congr ih => apply Red.congr1 .refl .refl_congr ih
-  case subst_congr ih1 ih2 => apply Red.congr2 .subst .subst_congr1 .subst_congr2 ih1 ih2
-  case phi_congr ih1 ih2 ih3 => apply Red.congr3 .phi .phi_congr1 .phi_congr2 .phi_congr3 ih1 ih2 ih3
-  case eq_congr ih1 ih2 ih3 => apply Red.congr3 .eq .eq_congr1 .eq_congr2 .eq_congr3 ih1 ih2 ih3
-  case conv_congr ih1 ih2 => apply Red.congr2 (λ t1 t2 => .conv t1 t2 _) .conv_congr1 .conv_congr2 ih1 ih2
+--   theorem to_red : s =β> t -> s -β>* t := by
+--   intro h
+--   induction h
+--   case bound => apply Term.Red.refl
+--   case none => apply Term.Red.refl
+--   case const => apply Term.Red.refl
+--   case beta A _A' b b' t t' m _ _ _ _ih1 ih2 ih3 =>
+--     have r1 := Red.congr2 (λ b t => .app m (.lam m A b) t)
+--       (by {
+--         intro t1 t2 t1' h; simp
+--         apply Red.app_congr1; apply Red.lam_congr2; apply h
+--       })
+--       (by {
+--         intro t1 t2 t2' h; simp
+--         apply Red.app_congr2; apply h
+--       })
+--       ih2 ih3
+--     simp at r1
+--     apply Red.trans_flip; apply r1; constructor
+--   case proj1 B _B' t t' s _s' _ _ _ _ih1 ih2 _ih3 =>
+--     have r1 := Red.congr1 (λ t => .fst (.pair B t s))
+--       (by {
+--         intro t t' h; simp
+--         apply Red.fst_congr; apply Red.pair_congr2; apply h
+--       })
+--       ih2
+--     simp at r1
+--     apply Red.trans_flip; apply r1; constructor
+--   case proj2 B _B' t _t' s s' _ _ _ _ih1 _ih2 ih3 =>
+--     have r1 := Red.congr1 (λ s => .snd (.pair B t s))
+--       (by {
+--         intro t t' h; simp
+--         apply Red.snd_congr; apply Red.pair_congr3; apply h
+--       })
+--       ih3
+--     simp at r1
+--     apply Red.trans_flip; apply r1; constructor
+--   -- case substelim B B' t t' _ _ ih1 ih2 =>
+--   --   have r1 := Red.congr2 (λ B t => .subst B (.refl t))
+--   --     (by {
+--   --       intro t1 t2 t1' h; simp
+--   --       apply Red.subst_congr1; apply h
+--   --     })
+--   --     (by {
+--   --       intro t1 t2 t2' h; simp
+--   --       apply Red.subst_congr2; apply Red.refl_congr; apply h
+--   --     })
+--   --     ih1 ih2
+--   --   simp at r1
+--   --   apply Red.trans_flip; apply r1; constructor
+--   -- case conv_lam B B' A2 A2' t t' m A1 n _ _ ih1 ih2 ih3 ih4 =>
+--   --   apply Red.trans; apply Red.congr1 (λ A2 => (all m A1 B).conv (lam m A2 t) n)
+--   --   intro t1 t1' h; apply Red.conv_congr2; apply Red.lam_congr1; apply h
+--   --   apply ih3;
+--   --   apply RedStar.step; apply Red.conv_lam
+--   --   apply Red.congr2 (λ B t => lam m A2' (conv B t n))
+--   --   intro t1 t2 t1' h; apply Red.lam_congr2; apply Red.conv_congr1; apply h
+--   --   intro t1 t2 t2' h; apply Red.lam_congr2; apply Red.conv_congr2; apply h
+--   --   apply ih2; apply ih4
+--   -- case conv_pair T T' t t' s s' n _ _ _ ih1 ih2 ih3 =>
+--   --   apply RedStar.step; constructor
+--   --   apply Red.congr3 (λ T t s => pair T t s)
+--   --   intro t1 t2 t3 t1' h; apply Red.pair_congr1; apply h
+--   --   intro t1 t2 t3 t2' h; apply Red.pair_congr2; apply h
+--   --   intro t1 t2 t3 t3' h; apply Red.pair_congr3; apply h
+--   --   apply ih1; apply ih2; apply ih3
+--   -- case conv_refl A A' t t' n _ _ ih1 ih2 =>
+--   --   apply RedStar.step; constructor
+--   --   apply Red.congr2 (λ A t => Term.refl (conv A t n))
+--   --   intro t1 t2 t1' h; apply Red.refl_congr; apply Red.conv_congr1; apply h
+--   --   intro t1 t2 t2' h; apply Red.refl_congr; apply Red.conv_congr2; apply h
+--   --   apply ih1; apply ih2
+--   case conv_all A A' B B' K m n _ _ ih1 ih2 =>
+--     apply RedStar.step; constructor
+--     apply Red.congr2 (λ A B => all m A B)
+--     intro t1 t2 t1' h; apply Red.all_congr1; apply h
+--     intro t1 t2 t2' h; apply Red.all_congr2; apply h
+--     apply ih1; apply ih2
+--   case conv_prod A A' B B' n _ _ ih1 ih2 =>
+--     apply RedStar.step; constructor
+--     apply Red.congr2 (λ A B => prod A B)
+--     intro t1 t2 t1' h; apply Red.prod_congr1; apply h
+--     intro t1 t2 t2' h; apply Red.prod_congr2; apply h
+--     apply ih1; apply ih2
+--   case conv_eq A A' a a' b b' n _ _ _ ih1 ih2 ih3 =>
+--     apply RedStar.step; constructor
+--     apply Red.congr3 (λ A a b => eq A a b)
+--     intro t1 t2 t3 t1' h; apply Red.eq_congr1; apply h
+--     intro t1 t2 t3 t2' h; apply Red.eq_congr2; apply h
+--     intro t1 t2 t3 t3' h; apply Red.eq_congr3; apply h
+--     apply ih1; apply ih2; apply ih3
+--   case lam_congr ih1 ih2 => apply Red.congr2 (.lam _) .lam_congr1 .lam_congr2 ih1 ih2
+--   case app_congr ih1 ih2 => apply Red.congr2 (.app _) .app_congr1 .app_congr2 ih1 ih2
+--   case all_congr ih1 ih2 => apply Red.congr2 (.all _) .all_congr1 .all_congr2 ih1 ih2
+--   case pair_congr ih1 ih2 ih3 => apply Red.congr3 .pair .pair_congr1 .pair_congr2 .pair_congr3 ih1 ih2 ih3
+--   case fst_congr ih => apply Red.congr1 .fst .fst_congr ih
+--   case snd_congr ih => apply Red.congr1 .snd .snd_congr ih
+--   case prod_congr ih1 ih2 => apply Red.congr2 .prod .prod_congr1 .prod_congr2 ih1 ih2
+--   case refl_congr ih => apply Red.congr1 .refl .refl_congr ih
+--   case subst_congr ih1 ih2 => apply Red.congr2 .subst .subst_congr1 .subst_congr2 ih1 ih2
+--   case phi_congr ih1 ih2 ih3 => apply Red.congr3 .phi .phi_congr1 .phi_congr2 .phi_congr3 ih1 ih2 ih3
+--   case eq_congr ih1 ih2 ih3 => apply Red.congr3 .eq .eq_congr1 .eq_congr2 .eq_congr3 ih1 ih2 ih3
+--   case conv_congr ih1 ih2 => apply Red.congr2 (λ t1 t2 => .conv t1 t2 _) .conv_congr1 .conv_congr2 ih1 ih2
+--   repeat sorry
 
-  theorem to_redstar : s =β>* t -> s -β>* t := by
-  intro h
-  induction h
-  case _ => apply Red.refl
-  case _ h _ ih => apply Red.trans (to_red h) ih
+--   theorem to_redstar : s =β>* t -> s -β>* t := by
+--   intro h
+--   induction h
+--   case _ => apply Red.refl
+--   case _ h _ ih => apply Red.trans (to_red h) ih
 
-  theorem subst_same σ : s =β> t -> [σ]s =β> [σ]t := by
-  intro h
-  induction h generalizing σ
-  case bound _ n => simp
-  case none => simp
-  case const => simp
-  case beta A A' b b' t t' m _ _ _ ih1 ih2 ih3 =>
-    have h3 := @ParRed.beta ([σ]A) ([σ]A') ([^σ]b) ([^σ]b') ([σ]t) ([σ]t') m
-    simp at *; apply h3
-    apply ih1 σ
-    replace ih2 := ih2 (^σ)
-    simp at ih2; apply ih2
-    apply ih3 σ
-  case proj1 B B' t t' s s' _ _ _ ih1 ih2 ih3 =>
-    have h3 := @ParRed.proj1 ([σ]B) ([σ]B') ([σ]t) ([σ]t') ([σ]s) ([σ]s')
-    simp at *; apply h3
-    apply ih1 σ; apply ih2 σ; apply ih3 σ
-  case proj2 B B' t t' s s' _ _ _ ih1 ih2 ih3 =>
-    have h3 := @ParRed.proj2 ([σ]B) ([σ]B') ([σ]t) ([σ]t') ([σ]s) ([σ]s')
-    simp at *; apply h3
-    apply ih1 σ; apply ih2 σ; apply ih3 σ
-  case substelim B B' t t' _ _ ih1 ih2 =>
-    have h3 := @ParRed.substelim ([σ]B) ([σ]B') ([σ]t) ([σ]t')
-    simp at *; apply h3
-    apply ih1 σ; apply ih2 σ
-  case lam_congr ih1 ih2 =>
-    simp; constructor; apply ih1 σ
-    replace ih2 := ih2 (^σ)
-    simp at ih2; exact ih2
-  case all_congr ih1 ih2 =>
-    simp; constructor; apply ih1 σ
-    replace ih2 := ih2 (^σ)
-    simp at ih2; exact ih2
-  case prod_congr ih1 ih2 =>
-    simp; constructor; apply ih1 σ
-    replace ih2 := ih2 (^σ)
-    simp at ih2; exact ih2
-  case conv_lam ih1 ih2 ih3 =>
-    simp; constructor
-    replace ih1 := ih1 (^σ)
-    simp at ih1; exact ih1
-    apply ih2 σ
-    replace ih3 := ih3 (^σ)
-    simp at ih3; exact ih3
-  case conv_pair ih1 ih2 ih3 =>
-    simp; constructor; apply ih1 _; apply ih2 _; apply ih3 _
-  case conv_all ih1 ih2 =>
-    simp; constructor; apply ih1 σ
-    replace ih2 := ih2 (^σ)
-    simp at ih2; exact ih2
-  case conv_prod ih1 ih2 =>
-    simp; constructor; apply ih1 σ
-    replace ih2 := ih2 (^σ)
-    simp at ih2; exact ih2
-  all_goals try (
-    case _ ih1 => simp at *; constructor; apply ih1 σ
-  )
-  all_goals try (
-    case _ ih1 ih2 => simp at *; constructor; apply ih1 σ; apply ih2 σ
-  )
-  all_goals try (
-    case _ ih1 ih2 ih3 => simp at *; constructor; apply ih1 σ; apply ih2 σ; apply ih3 σ
-  )
+--   theorem subst_same σ : s =β> t -> [σ]s =β> [σ]t := by
+--   intro h
+--   induction h generalizing σ
+--   case bound _ n => simp
+--   case none => simp
+--   case const => simp
+--   case beta A A' b b' t t' m _ _ _ ih1 ih2 ih3 =>
+--     have h3 := @ParRed.beta ([σ]A) ([σ]A') ([^σ]b) ([^σ]b') ([σ]t) ([σ]t') m
+--     simp at *; apply h3
+--     apply ih1 σ
+--     replace ih2 := ih2 (^σ)
+--     simp at ih2; apply ih2
+--     apply ih3 σ
+--   case proj1 B B' t t' s s' _ _ _ ih1 ih2 ih3 =>
+--     have h3 := @ParRed.proj1 ([σ]B) ([σ]B') ([σ]t) ([σ]t') ([σ]s) ([σ]s')
+--     simp at *; apply h3
+--     apply ih1 σ; apply ih2 σ; apply ih3 σ
+--   case proj2 B B' t t' s s' _ _ _ ih1 ih2 ih3 =>
+--     have h3 := @ParRed.proj2 ([σ]B) ([σ]B') ([σ]t) ([σ]t') ([σ]s) ([σ]s')
+--     simp at *; apply h3
+--     apply ih1 σ; apply ih2 σ; apply ih3 σ
+--   case substelim B B' t t' _ _ ih1 ih2 =>
+--     have h3 := @ParRed.substelim ([σ]B) ([σ]B') ([σ]t) ([σ]t')
+--     simp at *; apply h3
+--     apply ih1 σ; apply ih2 σ
+--   case lam_congr ih1 ih2 =>
+--     simp; constructor; apply ih1 σ
+--     replace ih2 := ih2 (^σ)
+--     simp at ih2; exact ih2
+--   case all_congr ih1 ih2 =>
+--     simp; constructor; apply ih1 σ
+--     replace ih2 := ih2 (^σ)
+--     simp at ih2; exact ih2
+--   case prod_congr ih1 ih2 =>
+--     simp; constructor; apply ih1 σ
+--     replace ih2 := ih2 (^σ)
+--     simp at ih2; exact ih2
+--   case conv_lam ih1 ih2 ih3 =>
+--     simp; constructor
+--     replace ih1 := ih1 (^σ)
+--     simp at ih1; exact ih1
+--     apply ih2 σ
+--     replace ih3 := ih3 (^σ)
+--     simp at ih3; exact ih3
+--   case conv_pair ih1 ih2 ih3 =>
+--     simp; constructor; apply ih1 _; apply ih2 _; apply ih3 _
+--   case conv_all ih1 ih2 =>
+--     simp; constructor; apply ih1 σ
+--     replace ih2 := ih2 (^σ)
+--     simp at ih2; exact ih2
+--   case conv_prod ih1 ih2 =>
+--     simp; constructor; apply ih1 σ
+--     replace ih2 := ih2 (^σ)
+--     simp at ih2; exact ih2
+--   all_goals try (
+--     case _ ih1 => simp at *; constructor; apply ih1 σ
+--   )
+--   all_goals try (
+--     case _ ih1 ih2 => simp at *; constructor; apply ih1 σ; apply ih2 σ
+--   )
+--   all_goals try (
+--     case _ ih1 ih2 ih3 => simp at *; constructor; apply ih1 σ; apply ih2 σ; apply ih3 σ
+--   )
 
-  theorem subst_lift_replace σ τ :
-    (∀ n t, σ n = .replace t -> ∃ t', τ n = .replace t' ∧ t =β> t') ->
-    ∀ n t, ^σ n = .replace t -> ∃ t', ^τ n = .replace t' ∧ t =β> t'
-  := by
-  intro h1 n t h2
-  cases n <;> simp at *
-  case _ n =>
-    unfold Subst.compose at *; simp at *
-    generalize ydef : σ n = y at *
-    cases y <;> simp at *
-    case _ q =>
-      replace h1 := h1 n q ydef
-      cases h1
-      case _ w h1 =>
-        rw [h1.1]; simp
-        subst h2; apply subst_same; apply h1.2
+--   theorem subst_lift_replace σ τ :
+--     (∀ n t, σ n = .replace t -> ∃ t', τ n = .replace t' ∧ t =β> t') ->
+--     ∀ n t, ^σ n = .replace t -> ∃ t', ^τ n = .replace t' ∧ t =β> t'
+--   := by
+--   intro h1 n t h2
+--   cases n <;> simp at *
+--   case _ n =>
+--     unfold Subst.compose at *; simp at *
+--     generalize ydef : σ n = y at *
+--     cases y <;> simp at *
+--     case _ q =>
+--       replace h1 := h1 n q ydef
+--       cases h1
+--       case _ w h1 =>
+--         rw [h1.1]; simp
+--         subst h2; apply subst_same; apply h1.2
 
-  theorem subst (σ τ : Subst Term) :
-    (∀ n t, σ n = .replace t -> ∃ t', τ n = .replace t' ∧ t =β> t') ->
-    (∀ n k, σ n = .rename k -> τ n = .rename k) ->
-    s =β> t -> [σ]s =β> [τ]t
-  := by
-  intro h1 h2 r
-  induction r generalizing σ τ
-  case bound _ n =>
-    simp; generalize ydef : σ n = y at *
-    cases y <;> simp
-    case _ i => rw [h2 n i]; simp; rw [ydef]
-    case _ t =>
-      replace h1 := h1 n t ydef
-      cases h1
-      case _ t' h1 =>
-        rw [h1.1]; simp; apply h1.2
-  case none => simp
-  case const => simp
-  case beta A A' b b' t t' m _ _ _ ih1 ih2 ih3 =>
-    have h3 := @ParRed.beta ([σ]A) ([τ]A') ([^σ]b) ([^τ]b') ([σ]t) ([τ]t') m
-    simp at *; apply h3
-    apply ih1 _ _ h1 h2
-    replace ih2 := ih2 (^σ) (^τ) (subst_lift_replace _ _ h1) (Red.subst_lift_rename _ _ h2)
-    simp at ih2; apply ih2
-    apply ih3 _ _ h1 h2
-  case proj1 B B' t t' s s' _ _ _ ih1 ih2 ih3 =>
-    have h3 := @ParRed.proj1 ([σ]B) ([τ]B') ([σ]t) ([τ]t') ([σ]s) ([τ]s')
-    simp at *; apply h3
-    apply ih1 _ _ h1 h2; apply ih2 _ _ h1 h2; apply ih3 _ _ h1 h2
-  case proj2 B B' t t' s s' _ _ _ ih1 ih2 ih3 =>
-    have h3 := @ParRed.proj2 ([σ]B) ([τ]B') ([σ]t) ([τ]t') ([σ]s) ([τ]s')
-    simp at *; apply h3
-    apply ih1 _ _ h1 h2; apply ih2 _ _ h1 h2; apply ih3 _ _ h1 h2
-  case substelim B B' t t' _ _ ih1 ih2 =>
-    have h3 := @ParRed.substelim ([σ]B) ([τ]B') ([σ]t) ([τ]t')
-    simp at *; apply h3
-    apply ih1 _ _ h1 h2; apply ih2 _ _ h1 h2
-  case conv_lam B B' A2 A2' t t' m A1 n _ _ _ ih1 ih2 ih3 =>
-    have h3 := @ParRed.conv_lam ([^σ]B) ([^τ]B') ([σ]A2) ([τ]A2') ([^σ]t) ([^τ]t') m ([σ]A1) n
-    simp at *; apply h3
-    replace ih1 := ih1 (^σ) (^τ) (subst_lift_replace _ _ h1) (Red.subst_lift_rename _ _ h2)
-    simp at ih1; apply ih1
-    apply ih2 _ _ h1 h2
-    replace ih3 := ih3 (^σ) (^τ) (subst_lift_replace _ _ h1) (Red.subst_lift_rename _ _ h2)
-    simp at ih3; apply ih3
-  case conv_pair T T' t t' s s' n _ _ _ ih1 ih2 ih3 =>
-    have h3 := @ParRed.conv_pair ([σ]T) ([τ]T') ([σ]t) ([τ]t') ([σ]s) ([τ]s') n
-    simp at *; apply h3
-    apply ih1 _ _ h1 h2; apply ih2 _ _ h1 h2; apply ih3 _ _ h1 h2
-  case conv_all A A' B B' K m n _ _ ih1 ih2 =>
-    have h3 := @ParRed.conv_all ([σ]A) ([τ]A') ([^σ]B) ([^τ]B') K m
-    simp at *; apply h3
-    apply ih1 _ _ h1 h2
-    replace ih2 := ih2 (^σ) (^τ) (subst_lift_replace _ _ h1) (Red.subst_lift_rename _ _ h2)
-    simp at ih2; apply ih2
-  case conv_prod A A' B B' n _ _ ih1 ih2 =>
-    have h3 := @ParRed.conv_prod ([σ]A) ([τ]A') ([^σ]B) ([^τ]B')
-    simp at *; apply h3
-    apply ih1 _ _ h1 h2
-    replace ih2 := ih2 (^σ) (^τ) (subst_lift_replace _ _ h1) (Red.subst_lift_rename _ _ h2)
-    simp at ih2; apply ih2
-  case lam_congr ih1 ih2 =>
-    simp; constructor; apply ih1 _ _ h1 h2
-    replace ih2 := ih2 (^σ) (^τ) (subst_lift_replace _ _ h1) (Red.subst_lift_rename _ _ h2)
-    simp at ih2; exact ih2
-  case all_congr ih1 ih2 =>
-    simp; constructor; apply ih1 _ _ h1 h2
-    replace ih2 := ih2 (^σ) (^τ) (subst_lift_replace _ _ h1) (Red.subst_lift_rename _ _ h2)
-    simp at ih2; exact ih2
-  case prod_congr ih1 ih2 =>
-    simp; constructor; apply ih1 _ _ h1 h2
-    replace ih2 := ih2 (^σ) (^τ) (subst_lift_replace _ _ h1) (Red.subst_lift_rename _ _ h2)
-    simp at ih2; exact ih2
-  all_goals try (
-    case _ ih1 =>
-    simp; constructor; apply ih1 _ _ h1 h2
-  )
-  all_goals try (
-    case _ ih1 ih2 =>
-    simp; constructor; apply ih1 _ _ h1 h2; apply ih2 _ _ h1 h2
-  )
-  all_goals try (
-    case _ ih1 ih2 ih3 =>
-    simp; constructor; apply ih1 _ _ h1 h2; apply ih2 _ _ h1 h2; apply ih3 _ _ h1 h2
-  )
+--   theorem subst (σ τ : Subst Term) :
+--     (∀ n t, σ n = .replace t -> ∃ t', τ n = .replace t' ∧ t =β> t') ->
+--     (∀ n k, σ n = .rename k -> τ n = .rename k) ->
+--     s =β> t -> [σ]s =β> [τ]t
+--   := by
+--   intro h1 h2 r
+--   induction r generalizing σ τ
+--   case bound _ n =>
+--     simp; generalize ydef : σ n = y at *
+--     cases y <;> simp
+--     case _ i => rw [h2 n i]; simp; rw [ydef]
+--     case _ t =>
+--       replace h1 := h1 n t ydef
+--       cases h1
+--       case _ t' h1 =>
+--         rw [h1.1]; simp; apply h1.2
+--   case none => simp
+--   case const => simp
+--   case beta A A' b b' t t' m _ _ _ ih1 ih2 ih3 =>
+--     have h3 := @ParRed.beta ([σ]A) ([τ]A') ([^σ]b) ([^τ]b') ([σ]t) ([τ]t') m
+--     simp at *; apply h3
+--     apply ih1 _ _ h1 h2
+--     replace ih2 := ih2 (^σ) (^τ) (subst_lift_replace _ _ h1) (Red.subst_lift_rename _ _ h2)
+--     simp at ih2; apply ih2
+--     apply ih3 _ _ h1 h2
+--   case proj1 B B' t t' s s' _ _ _ ih1 ih2 ih3 =>
+--     have h3 := @ParRed.proj1 ([σ]B) ([τ]B') ([σ]t) ([τ]t') ([σ]s) ([τ]s')
+--     simp at *; apply h3
+--     apply ih1 _ _ h1 h2; apply ih2 _ _ h1 h2; apply ih3 _ _ h1 h2
+--   case proj2 B B' t t' s s' _ _ _ ih1 ih2 ih3 =>
+--     have h3 := @ParRed.proj2 ([σ]B) ([τ]B') ([σ]t) ([τ]t') ([σ]s) ([τ]s')
+--     simp at *; apply h3
+--     apply ih1 _ _ h1 h2; apply ih2 _ _ h1 h2; apply ih3 _ _ h1 h2
+--   case substelim B B' t t' _ _ ih1 ih2 =>
+--     have h3 := @ParRed.substelim ([σ]B) ([τ]B') ([σ]t) ([τ]t')
+--     simp at *; apply h3
+--     apply ih1 _ _ h1 h2; apply ih2 _ _ h1 h2
+--   case conv_lam B B' A2 A2' t t' m A1 n _ _ _ ih1 ih2 ih3 =>
+--     have h3 := @ParRed.conv_lam ([^σ]B) ([^τ]B') ([σ]A2) ([τ]A2') ([^σ]t) ([^τ]t') m ([σ]A1) n
+--     simp at *; apply h3
+--     replace ih1 := ih1 (^σ) (^τ) (subst_lift_replace _ _ h1) (Red.subst_lift_rename _ _ h2)
+--     simp at ih1; apply ih1
+--     apply ih2 _ _ h1 h2
+--     replace ih3 := ih3 (^σ) (^τ) (subst_lift_replace _ _ h1) (Red.subst_lift_rename _ _ h2)
+--     simp at ih3; apply ih3
+--   case conv_pair T T' t t' s s' n _ _ _ ih1 ih2 ih3 =>
+--     have h3 := @ParRed.conv_pair ([σ]T) ([τ]T') ([σ]t) ([τ]t') ([σ]s) ([τ]s') n
+--     simp at *; apply h3
+--     apply ih1 _ _ h1 h2; apply ih2 _ _ h1 h2; apply ih3 _ _ h1 h2
+--   case conv_all A A' B B' K m n _ _ ih1 ih2 =>
+--     have h3 := @ParRed.conv_all ([σ]A) ([τ]A') ([^σ]B) ([^τ]B') K m
+--     simp at *; apply h3
+--     apply ih1 _ _ h1 h2
+--     replace ih2 := ih2 (^σ) (^τ) (subst_lift_replace _ _ h1) (Red.subst_lift_rename _ _ h2)
+--     simp at ih2; apply ih2
+--   case conv_prod A A' B B' n _ _ ih1 ih2 =>
+--     have h3 := @ParRed.conv_prod ([σ]A) ([τ]A') ([^σ]B) ([^τ]B')
+--     simp at *; apply h3
+--     apply ih1 _ _ h1 h2
+--     replace ih2 := ih2 (^σ) (^τ) (subst_lift_replace _ _ h1) (Red.subst_lift_rename _ _ h2)
+--     simp at ih2; apply ih2
+--   case lam_congr ih1 ih2 =>
+--     simp; constructor; apply ih1 _ _ h1 h2
+--     replace ih2 := ih2 (^σ) (^τ) (subst_lift_replace _ _ h1) (Red.subst_lift_rename _ _ h2)
+--     simp at ih2; exact ih2
+--   case all_congr ih1 ih2 =>
+--     simp; constructor; apply ih1 _ _ h1 h2
+--     replace ih2 := ih2 (^σ) (^τ) (subst_lift_replace _ _ h1) (Red.subst_lift_rename _ _ h2)
+--     simp at ih2; exact ih2
+--   case prod_congr ih1 ih2 =>
+--     simp; constructor; apply ih1 _ _ h1 h2
+--     replace ih2 := ih2 (^σ) (^τ) (subst_lift_replace _ _ h1) (Red.subst_lift_rename _ _ h2)
+--     simp at ih2; exact ih2
+--   all_goals try (
+--     case _ ih1 =>
+--     simp; constructor; apply ih1 _ _ h1 h2
+--   )
+--   all_goals try (
+--     case _ ih1 ih2 =>
+--     simp; constructor; apply ih1 _ _ h1 h2; apply ih2 _ _ h1 h2
+--   )
+--   all_goals try (
+--     case _ ih1 ih2 ih3 =>
+--     simp; constructor; apply ih1 _ _ h1 h2; apply ih2 _ _ h1 h2; apply ih3 _ _ h1 h2
+--   )
 
-  theorem subst_beta : b =β> b' -> t =β> t' -> b β[t] =β> b' β[t'] := by
-  intro h1 h2
-  apply subst <;> simp [*]
-  case _ =>
-    intro n x h
-    cases n <;> simp at *
-    case _ => subst h; apply h2
-  case _ =>
-    intro n x h
-    cases n <;> simp at *
-    case _ => exact h
+--   theorem subst_beta : b =β> b' -> t =β> t' -> b β[t] =β> b' β[t'] := by
+--   intro h1 h2
+--   apply subst <;> simp [*]
+--   case _ =>
+--     intro n x h
+--     cases n <;> simp at *
+--     case _ => subst h; apply h2
+--   case _ =>
+--     intro n x h
+--     cases n <;> simp at *
+--     case _ => exact h
 
-  theorem complete : s =β> t -> t =β> pcompl s := by
-  intro h
-  induction h
-  case beta m _ _ _ _ _ _ =>
-    cases m <;> simp
-    all_goals (
-      apply subst
-      case _ =>
-        intro n t h; simp at *
-        cases n <;> simp at *
-        subst h; simp [*]
-      case _ =>
-        intro n k h; simp at *
-        cases n <;> simp at * <;> simp [*]
-      case _ => simp [*]
-    )
-  case proj1 => simp [*]
-  case proj2 => simp [*]
-  case substelim =>
-    simp; constructor; constructor;
-    all_goals simp [*]
-  case conv_lam ih1 ih2 ih3 ih4 =>
-    simp; constructor; apply ih3; constructor; apply ih2; apply ih4
-  case conv_pair ih1 ih2 ih3 =>
-    simp; constructor; apply ih1; apply ih2; apply ih3
-  case conv_refl ih1 ih2 =>
-    simp; constructor; constructor; apply ih1; apply ih2
-  case app_congr f f' a a' m h1 _h2 ih1 ih2 =>
-    cases m
-    case _ =>
-      cases f
-      all_goals (try constructor; apply ih1; apply ih2)
-      case _ m' _ _ =>
-      cases m' <;> simp at*
-      case _ =>
-        cases f' <;> cases h1
-        case _ r1 r2 =>
-          cases ih1
-          case _ h1 h2 =>
-            apply ParRed.beta; apply h1; apply h2; apply ih2
-      case _ => apply ParRed.app_congr <;> simp [*]
-      case _ => apply ParRed.app_congr <;> simp [*]
-    case _ =>
-      cases f
-      all_goals (try constructor; apply ih1; apply ih2)
-      case _ m' _ _ =>
-      cases m' <;> simp at *
-      case _ => apply ParRed.app_congr <;> simp [*]
-      case _ =>
-        cases f' <;> cases h1
-        case _ r1 r2 =>
-          cases ih1
-          case _ h1 h2 =>
-            apply ParRed.beta; apply h1; apply h2; apply ih2
-      case _ => apply ParRed.app_congr <;> simp [*]
-    case _ =>
-      cases f
-      all_goals (try constructor; apply ih1; apply ih2)
-      case _ m' _ _ =>
-      cases m' <;> simp at *
-      case _ => apply ParRed.app_congr <;> simp [*]
-      case _ => apply ParRed.app_congr <;> simp [*]
-      case _ =>
-        cases f' <;> cases h1
-        case _ r1 r2 =>
-          cases ih1
-          case _ h1 h2 =>
-            apply ParRed.beta; apply h1; apply h2; apply ih2
-  case fst_congr t t' h ih =>
-    cases t <;> simp at *
-    all_goals (try constructor; apply ih)
-    case pair B t s =>
-      cases t' <;> try cases h
-      case _ h1 h2 h3 =>
-        cases ih
-        case _ r1 r2 r3 =>
-          apply ParRed.proj1
-          apply r1; apply r2; apply r3
-  case snd_congr t t' h ih =>
-    cases t <;> simp at *
-    all_goals (try constructor; apply ih)
-    case pair B t s =>
-      cases t' <;> try cases h
-      case _ h1 h2 h3 =>
-        cases ih
-        case _ r1 r2 r3 =>
-          apply ParRed.proj2
-          apply r1; apply r2; apply r3
-  case subst_congr B B' e e' _h1 h2 ih1 ih2 =>
-    cases e <;> simp at *
-    all_goals (try constructor; apply ih1; apply ih2)
-    case _ e =>
-      cases e' <;> try cases h2
-      case _ h =>
-        cases ih2
-        case _ r =>
-          apply ParRed.substelim; apply ih1; apply r
-  case conv_congr A A' t t' n h1 h2 ih1 ih2 =>
-    cases t <;> simp at *
-    all_goals (try constructor; apply ih1; apply ih2)
-    case lam m1 u1 u2 =>
-      cases t' <;> try cases h2
-      case _ t1 t2 r1 h =>
-        cases ih2
-        case _ r2 r3 =>
-          cases A <;> simp [*]
-          all_goals (try constructor; apply ih1; constructor <;> simp [*])
-          case _ m2 v1 v2 =>
-            cases h1; cases ih1
-            case _  A' B' r4 r5 r6 r7 =>
-              sorry
-    case all => sorry
-    case prod => sorry
-    case pair => sorry
-    case refl => sorry
-    case eq => sorry
+--   theorem complete : s =β> t -> t =β> pcompl s := by
+--   intro h
+--   induction h
+--   case beta m _ _ _ _ _ _ =>
+--     cases m <;> simp
+--     all_goals (
+--       apply subst
+--       case _ =>
+--         intro n t h; simp at *
+--         cases n <;> simp at *
+--         subst h; simp [*]
+--       case _ =>
+--         intro n k h; simp at *
+--         cases n <;> simp at * <;> simp [*]
+--       case _ => simp [*]
+--     )
+--   case proj1 => simp [*]
+--   case proj2 => simp [*]
+--   case substelim =>
+--     simp; constructor; constructor;
+--     all_goals simp [*]
+--   case conv_lam ih1 ih2 ih3 ih4 =>
+--     simp; constructor; apply ih3; constructor; apply ih2; apply ih4
+--   case conv_pair ih1 ih2 ih3 =>
+--     simp; constructor; apply ih1; apply ih2; apply ih3
+--   case conv_refl ih1 ih2 =>
+--     simp; constructor; constructor; apply ih1; apply ih2
+--   case app_congr f f' a a' m h1 _h2 ih1 ih2 =>
+--     cases m
+--     case _ =>
+--       cases f
+--       all_goals (try constructor; apply ih1; apply ih2)
+--       case _ m' _ _ =>
+--       cases m' <;> simp at*
+--       case _ =>
+--         cases f' <;> cases h1
+--         case _ r1 r2 =>
+--           cases ih1
+--           case _ h1 h2 =>
+--             apply ParRed.beta; apply h1; apply h2; apply ih2
+--       case _ => apply ParRed.app_congr <;> simp [*]
+--       case _ => apply ParRed.app_congr <;> simp [*]
+--     case _ =>
+--       cases f
+--       all_goals (try constructor; apply ih1; apply ih2)
+--       case _ m' _ _ =>
+--       cases m' <;> simp at *
+--       case _ => apply ParRed.app_congr <;> simp [*]
+--       case _ =>
+--         cases f' <;> cases h1
+--         case _ r1 r2 =>
+--           cases ih1
+--           case _ h1 h2 =>
+--             apply ParRed.beta; apply h1; apply h2; apply ih2
+--       case _ => apply ParRed.app_congr <;> simp [*]
+--     case _ =>
+--       cases f
+--       all_goals (try constructor; apply ih1; apply ih2)
+--       case _ m' _ _ =>
+--       cases m' <;> simp at *
+--       case _ => apply ParRed.app_congr <;> simp [*]
+--       case _ => apply ParRed.app_congr <;> simp [*]
+--       case _ =>
+--         cases f' <;> cases h1
+--         case _ r1 r2 =>
+--           cases ih1
+--           case _ h1 h2 =>
+--             apply ParRed.beta; apply h1; apply h2; apply ih2
+--   case fst_congr t t' h ih =>
+--     cases t <;> simp at *
+--     all_goals (try constructor; apply ih)
+--     case pair B t s =>
+--       cases t' <;> try cases h
+--       case _ h1 h2 h3 =>
+--         cases ih
+--         case _ r1 r2 r3 =>
+--           apply ParRed.proj1
+--           apply r1; apply r2; apply r3
+--   case snd_congr t t' h ih =>
+--     cases t <;> simp at *
+--     all_goals (try constructor; apply ih)
+--     case pair B t s =>
+--       cases t' <;> try cases h
+--       case _ h1 h2 h3 =>
+--         cases ih
+--         case _ r1 r2 r3 =>
+--           apply ParRed.proj2
+--           apply r1; apply r2; apply r3
+--   case subst_congr B B' e e' _h1 h2 ih1 ih2 =>
+--     cases e <;> simp at *
+--     all_goals (try constructor; apply ih1; apply ih2)
+--     case _ e =>
+--       cases e' <;> try cases h2
+--       case _ h =>
+--         cases ih2
+--         case _ r =>
+--           apply ParRed.substelim; apply ih1; apply r
+--   case conv_congr A A' t t' n h1 h2 ih1 ih2 =>
+--     cases t <;> simp at *
+--     all_goals (try constructor; apply ih1; apply ih2)
+--     case lam m1 u1 u2 =>
+--       cases t' <;> try cases h2
+--       case _ t1 t2 r1 h =>
+--         cases ih2
+--         case _ r2 r3 =>
+--           cases A <;> simp [*]
+--           all_goals (try constructor; apply ih1; constructor <;> simp [*])
+--           case _ m2 v1 v2 =>
+--             cases h1; cases ih1
+--             case _  A' B' r4 r5 r6 r7 =>
+--               sorry
+--     case all => sorry
+--     case prod => sorry
+--     case pair => sorry
+--     case refl => sorry
+--     case eq => sorry
 
-  all_goals (try simp; constructor <;> simp [*])
-  all_goals (try simp)
+--   all_goals (try simp; constructor <;> simp [*])
+--   all_goals (try simp)
 
-  theorem strip : s =β> t1 -> s =β>* t2 -> ∃ t, t1 =β>* t ∧ t2 =β> t := by
-  intro h1 h2
-  induction h2 generalizing t1
-  case _ t' => exists t1; apply And.intro; apply refl; apply h1
-  case _ x y z r1 _r2 ih =>
-    have r3 := complete r1
-    replace ih := ih r3
-    cases ih
-    case _ w ih =>
-      replace _r3 := ParRedStar.step r3 ih.1
-      replace h1 := complete h1
-      replace r3 := ParRedStar.step h1 ih.1
-      exists w; apply And.intro; apply r3; apply ih.2
+--   theorem strip : s =β> t1 -> s =β>* t2 -> ∃ t, t1 =β>* t ∧ t2 =β> t := by
+--   intro h1 h2
+--   induction h2 generalizing t1
+--   case _ t' => exists t1; apply And.intro; apply refl; apply h1
+--   case _ x y z r1 _r2 ih =>
+--     have r3 := complete r1
+--     replace ih := ih r3
+--     cases ih
+--     case _ w ih =>
+--       replace _r3 := ParRedStar.step r3 ih.1
+--       replace h1 := complete h1
+--       replace r3 := ParRedStar.step h1 ih.1
+--       exists w; apply And.intro; apply r3; apply ih.2
 
-  theorem confluence : s =β>* t1 -> s =β>* t2 -> t1 ≡β≡ t2 := by
-  intro h1 h2
-  induction h1 generalizing t2
-  case _ z =>
-    exists t2; apply And.intro
-    apply h2; apply refl
-  case _ s y t1 r1 _r2 ih =>
-    have h3 := strip r1 h2
-    cases h3
-    case _ w h3 =>
-      replace ih := ih h3.1
-      cases ih
-      case _ q ih =>
-        exists q; apply And.intro
-        apply ih.1; apply ParRedStar.step
-        apply h3.2; apply ih.2
+--   theorem confluence : s =β>* t1 -> s =β>* t2 -> t1 ≡β≡ t2 := by
+--   intro h1 h2
+--   induction h1 generalizing t2
+--   case _ z =>
+--     exists t2; apply And.intro
+--     apply h2; apply refl
+--   case _ s y t1 r1 _r2 ih =>
+--     have h3 := strip r1 h2
+--     cases h3
+--     case _ w h3 =>
+--       replace ih := ih h3.1
+--       cases ih
+--       case _ q ih =>
+--         exists q; apply And.intro
+--         apply ih.1; apply ParRedStar.step
+--         apply h3.2; apply ih.2
 
-end ParRed
+-- end ParRed
 
-namespace ParRedConv
+-- namespace ParRedConv
 
-  theorem refl : A ≡β≡ A := by
-  induction A
-  all_goals (
-    apply Exists.intro; apply And.intro
-    apply ParRedStar.refl; apply ParRedStar.refl
-  )
+--   theorem refl : A ≡β≡ A := by
+--   induction A
+--   all_goals (
+--     apply Exists.intro; apply And.intro
+--     apply ParRedStar.refl; apply ParRedStar.refl
+--   )
 
-  theorem sym : A ≡β≡ B -> B ≡β≡ A := by
-  intro h
-  cases h
-  case _ C ih => exists C; simp [*]
+--   theorem sym : A ≡β≡ B -> B ≡β≡ A := by
+--   intro h
+--   cases h
+--   case _ C ih => exists C; simp [*]
 
-  theorem trans : A ≡β≡ B -> B ≡β≡ C -> A ≡β≡ C := by
-  intro h1 h2
-  cases h1
-  case _ C1 ih1 =>
-    cases h2
-    case _ C2 ih2 =>
-      have conf := ParRed.confluence ih1.2 ih2.1
-      cases conf
-      case _ Z ih =>
-        exists Z; apply And.intro
-        apply ParRed.trans ih1.1 ih.1
-        apply ParRed.trans ih2.2 ih.2
+--   theorem trans : A ≡β≡ B -> B ≡β≡ C -> A ≡β≡ C := by
+--   intro h1 h2
+--   cases h1
+--   case _ C1 ih1 =>
+--     cases h2
+--     case _ C2 ih2 =>
+--       have conf := ParRed.confluence ih1.2 ih2.1
+--       cases conf
+--       case _ Z ih =>
+--         exists Z; apply And.intro
+--         apply ParRed.trans ih1.1 ih.1
+--         apply ParRed.trans ih2.2 ih.2
 
-end ParRedConv
+-- end ParRedConv
 
 namespace Red
 
-  theorem confluence : s -β>* t1 -> s -β>* t2 -> t1 =β= t2 := by
-  intro h1 h2
-  replace h1 := ParRed.from_redstar h1
-  replace h2 := ParRed.from_redstar h2
-  have conf := ParRed.confluence h1 h2
-  cases conf
-  case _ t conf =>
-    exists t; apply And.intro
-    apply ParRed.to_redstar conf.1
-    apply ParRed.to_redstar conf.2
+  theorem confluence : s -β>* t1 -> s -β>* t2 -> t1 =β= t2 := by sorry
+  -- intro h1 h2
+  -- replace h1 := ParRed.from_redstar h1
+  -- replace h2 := ParRed.from_redstar h2
+  -- have conf := ParRed.confluence h1 h2
+  -- cases conf
+  -- case _ t conf =>
+  --   exists t; apply And.intro
+  --   apply ParRed.to_redstar conf.1
+  --   apply ParRed.to_redstar conf.2
 
 end Red
 
