WCCC/Proof.lean
@@ -1,120 +1,73 @@
 
 import Common
 import WCCC.Mode
+import WCCC.Ctx
 
 namespace WCCC
 
-  abbrev Ctx := List (Mode × Term)
-
-  inductive Conv : CvTerm -> Term -> Term -> Prop
-  | sym : Conv c t2 t1 -> Conv (.sym c) t1 t2
-  | trans : Conv c1 t1 t2 -> Conv c2 t2 t3 -> Conv (.trans c1 c2) t1 t3
-  | none : Conv .none .none .none
-  | const : Conv .const (.const K) (.const K)
-  | bound x : Conv (.bound x) (.bound K x) (.bound K x)
-  | all_congr : Conv c1 A1 A2 -> Conv c2 B1 B2 ->
-    Conv (.all_congr c1 c2) (.all m A1 B1) (.all m A2 B2)
-  | lam_congr : Conv c1 A1 A2 -> Conv c2 t1 t2 ->
-    Conv (.lam_congr c1 c2) (.lam m A1 t1) (.lam m A2 t2)
-  | lam_eta : Conv c (.lam m A t1) (Term.eta m A t2) ->
-    Conv (.lam_eta c) (.lam m A t1) t2
-  | lam_mf_erased : Conv c t1 t2 ->
-    Conv (.lam_mf_erased c) (.lam mf A1 t1) (.lam mf A2 t2)
-  | lam_m0_erased : Conv c t1 t2 ->
-    Conv (.lam_m0_erased c) (.lam m0 A t1) t2
-  | app_congr : Conv c1 f1 f2 -> Conv c2 a1 a2 ->
-    Conv (.app_congr c1 c2) (.app m f1 a1) (.app m f2 a2)
-  | app_beta :
-    Conv c (b β[t]) t2 ->
-    Conv (.app_beta c) (.app m (.lam m A b) t) t2
-  | app_m0_erased : Conv c t1 t2 ->
-    Conv (.app_m0_erased c) (.app m0 t1 a) t2
-  | prod_congr : Conv c1 A1 A2 -> Conv c2 B1 B2 ->
-    Conv (.prod_congr c1 c2) (.prod A1 B1) (.prod A2 B2)
-  | pair_congr : Conv c1 T1 T2 -> Conv c2 t1 t2 -> Conv c3 s1 s2 ->
-    Conv (.pair_congr c1 c2 c3) (.pair T1 t1 s1) (.pair T2 t2 s2)
-  | pair_erased : Conv c t1 t2 ->
-    Conv (.pair_erased c) (.pair T1 t1 s1) t2
-  | fst_congr : Conv c t1 t2 -> Conv (.fst_congr c) (.fst t1) (.fst t2)
-  | fst_erased : Conv c t1 t2 -> Conv (.fst_erased c) (.fst t1) t2
-  | snd_congr : Conv c t1 t2 -> Conv (.snd_congr c) (.snd t1) (.snd t2)
-  | snd_erased : Conv c t1 t2 -> Conv (.snd_erased c) (.snd t1) t2
-  | phi_erased : Conv c a1 t2 -> Conv (.phi_erased c) (.phi a1 b1 e1) t2
-  | phi_congr : Conv c1 a1 a2 -> Conv c2 b1 b2 -> Conv c3 e1 e2 ->
-    Conv (.phi_congr c1 c2 c3) (.phi a1 b1 e1) (.phi a2 b2 e2)
-  | eq_congr : Conv c1 A1 A2 -> Conv c2 a1 a2 -> Conv c3 b1 b2 ->
-    Conv (.eq_congr c1 c2 c3) (.eq A1 a1 b1) (.eq A2 a2 b2)
-  | refl_congr : Conv c t1 t2 -> Conv (.refl_congr c) (.refl t1) (.refl t2)
-  | refl_erased : Conv c (.lam mf .none (.bound .type 0)) t2 ->
-    Conv (.refl_erased c) (.refl t1) t2
-  | subst_congr : Conv c1 P1 P2 -> Conv c2 e1 e2 ->
-    Conv (.subst_congr c1 c2) (.subst P1 e1) (.subst P2 e2)
-  | subst_erased : Conv c e1 t2 -> Conv (.subst_erased c) (.subst P1 e1) t2
-  | conv_congr : Conv c1 x1 x2 -> Conv c2 y1 y2 ->
-    Conv (.conv_congr c1 c2) (.conv x1 y1 z1) (.conv x2 y2 z2)
-  | conv_erased : Conv c t1 t2 -> Conv (.conv_erased c) (.conv A1 t1 c1) t2
-
-  notation:100 c:33 " : " A:32 " === " B:31 => Conv c A B
-
-  inductive Proof : Ctx -> Mode -> Term -> Term -> Prop
-  | ax : Proof Γ mt ★ □
+  inductive Proof : Ctx -> Term -> Term -> Prop
+  | ax :
+    ∀ (f : Nat -> Const), (∀ x, Proof Γ (Γ d@ x) (.const (f x))) ->
+    Proof Γ ★ □
   | var :
-    List.getD Γ x (mf, .none) = (m1, [r#(Term.Pn (x + 1))]A) ->
-    Proof (List.drop (x + 1) Γ) mt ([r#(Term.Pn (x + 1))]A) (.const K) ->
-    m1 ∈ m2 ->
-    Proof Γ m2 (.bound K x) A
+    Proof Γ (Γ d@ x) (.const K) ->
+    Proof Γ (.bound K x) (Γ d@ x)
   | pi :
-    Proof Γ mt A (Mode.dom m K) ->
-    Proof ((mt, A)::Γ) mt B (Mode.codom m) ->
-    Proof Γ mt (.all m A B) (Mode.codom m)
+    Proof Γ A (Mode.dom m K) ->
+    Proof (A::Γ) B (Mode.codom m) ->
+    Proof Γ (.all m A B) (Mode.codom m)
   | lam :
-    Proof Γ mt A (Mode.dom m2 K) ->
-    Proof ((m2, A)::Γ) m1 t B ->
-    Proof ((mt, A)::Γ) mt B (Mode.codom m2) ->
-    Proof Γ m1 (.lam m2 A t) (.all m2 A B)
+    Proof Γ (.all m A B) (Mode.codom m) ->
+    Proof (A::Γ) t B ->
+    Proof Γ (.lam m A t) (.all m A B)
   | app :
-    Proof Γ m1 f (.all m2 A B) ->
-    Proof Γ (m1*m2) a A ->
-    Proof Γ m1 (.app m2 f a) (B β[a])
+    Proof Γ f (.all m A B) ->
+    Proof Γ a A ->
+    Proof Γ (.app m f a) (B β[a])
   | prod :
-    Proof Γ mt A ★ ->
-    Proof ((mt, A)::Γ) mt B ★ ->
-    Proof Γ mt (.prod A B) ★
+    Proof Γ A ★ ->
+    Proof (A::Γ) B ★ ->
+    Proof Γ (.prod A B) ★
   | pair :
-    Proof Γ mt B (.all mf A ★) ->
-    Proof Γ m t A ->
-    Proof Γ m0 s (B β[t]) ->
-    Proof Γ m (.pair B t s) (.prod A B)
+    Proof (A::Γ) B ★ ->
+    Proof Γ t A ->
+    Proof Γ s (B β[t]) ->
+    t.erase =β{n}= s.erase ->
+    Proof Γ (.pair B t s) (.prod A B)
   | fst :
-    Proof Γ m t (.prod A B) ->
-    Proof Γ m (.fst t) A
+    Proof Γ t (.prod A B) ->
+    Proof Γ (.fst t) A
   | snd :
-    Proof Γ m0 t (.prod A B) ->
-    m0 ∈ m ->
-    Proof Γ m (.snd t) (B β[.fst t])
+    Proof Γ t (.prod A B) ->
+    Proof Γ (.snd t) (B β[.fst t])
   | eq :
-    Proof Γ mt A ★ ->
-    Proof Γ mt a A ->
-    Proof Γ mt b A ->
-    Proof Γ mt (.eq A a b) ★
+    Proof Γ A ★ ->
+    Proof Γ a A ->
+    Proof Γ b A ->
+    Proof Γ (.eq A a b) ★
   | refl :
-    Proof Γ m0 t A ->
-    Proof Γ m (.refl t) (.eq A t t)
+    Proof Γ t A ->
+    Proof Γ (.refl t) (.eq A t t)
   | subst :
-    Proof Γ m e (.eq A a b) ->
-    Proof Γ mt P (.all mt A ★) ->
-    Proof Γ m (.subst P e) (.all mf (.app mt P a) (.app mt P b))
+    Proof Γ e (.eq A a b) ->
+    Proof Γ Pr (.all mt A ★) ->
+    Proof Γ (.subst Pr e) (.all mf (.app mt Pr a) (.app mt Pr b))
   | phi :
-    Proof Γ m a A ->
-    Proof Γ m0 b (.prod A B) ->
-    Proof Γ m0 e (.eq A a (.fst b)) ->
-    Proof Γ m (.phi a b e) (.prod A B)
-  | conv :
-    Proof Γ m t A ->
-    Proof Γ mt B K ->
-    c : A === B ->
-    Proof Γ m (.conv B t c) B
+    Proof Γ a A ->
+    Proof Γ b (.prod A B) ->
+    Proof Γ e (.eq A a (.fst b)) ->
+    Proof Γ (.phi a b e) (.prod A B)
+  | iconv :
+    Proof Γ t A ->
+    Proof Γ B K ->
+    A =β= B ->
+    Proof Γ t B
+  | econv :
+    Proof Γ t A ->
+    Proof Γ B K ->
+    A.erase =β{n}= B.erase ->
+    Proof Γ (.conv B t n) B
 
-  notation:170 Γ:170 " ⊢[" m:170 "] " t:170 " : " A:170 => Proof Γ m t A
+  notation:170 Γ:170 " ⊢ " t:170 " : " A:170 => Proof Γ t A
 
 end WCCC
