Common.lean
@@ -5,4 +5,5 @@ import Common.Term.Normal
 import Common.Term.Classify
 import Common.Term.Substitution
 import Common.Term.Reduction
+import Common.Term.Erasure
 import Common.Util
