Common/Term/Erasure.lean
@@ -1,0 +1,28 @@
+import Common.Term
+import Common.Term.Substitution
+import Common.Term.Reduction
+
+namespace Term
+
+  def erase : Term -> Term
+  | .bound K i => .bound K i
+  | .none => .none
+  | .const K => .const K
+  | .lam m0 _ t => erase t
+  | .lam mf _ t => .lam mf .none (erase t)
+  | .lam mt A t => .lam mt (erase A) (erase t)
+  | .app m0 f _ => erase f
+  | .app mf f a => .app mf (erase f) (erase a)
+  | .app mt f a => .app mt (erase f) (erase a)
+  | .all m A B => .all m (erase A) (erase B)
+  | .pair n _ t _ => erase t
+  | .fst t => erase t
+  | .snd t => erase t
+  | .prod A B => .prod (erase A) (erase B)
+  | .refl _ => .lam mf .none (.bound .type 0)
+  | .subst _ e => erase e
+  | .phi a _ _ => erase a
+  | .eq A a b => .eq (erase A) (erase a) (erase b)
+  | .conv _ t _ => erase t
+
+end Term
