Fomega/Basic/Normalization.lean
@@ -1,0 +1,88 @@
+import Common
+import Fomega.Ctx
+import Fomega.Proof
+import Fomega.PreProof
+import Fomega.Basic.Weaken
+import Fomega.Basic.Substitution
+import Fomega.Basic.Inversion
+import Fomega.Basic.Classification
+import Fomega.Basic.Preservation
+
+namespace Fomega.Proof
+
+  abbrev Cand := Term -> Prop
+
+  def PossibleRedex : Term -> Bool
+  | .app _ _ _ => true
+  | _ => false
+
+  structure Reducible (P : Cand) : Prop where
+    normal : ∀ t, P t -> Term.SN t
+    preserve : ∀ t t', P t -> t -β> t' -> P t'
+    expand : ∀ t, PossibleRedex t -> (∀ t', t -β> t' -> P t') -> P t
+
+  def L (ty : Term) (rho : Nat -> Cand) : Cand :=
+    match ty with
+    | .bound .kind x => rho x
+    | .all mf A B => λ f => ∀ a, L A rho a -> L B rho (.app mf f a)
+    | _ => λ _ => False
+
+  def EL (Γ : Ctx) (f : Nat -> Const) (rho : Nat -> Cand) (σ : Subst Term) : Prop :=
+    ∀ x, L (Γ d@ x) rho ([σ].bound (f x) x)
+
+  def Admissible (rho : Nat -> Cand) := ∀ x, Reducible (rho x)
+
+  def stream_to_subst : (Nat -> Term) -> Subst Term
+  | s, n => .replace (s n)
+
+  prefix:15 ":s2s:" => stream_to_subst
+
+  -- Facts about Reducible Sets
+
+  theorem reducible_sn : Reducible Term.SN := by
+  constructor; simp
+  case _ =>
+    intro t t' h r
+    cases h; case _ h => apply h _ r
+  case _ =>
+    intro t _ h
+    constructor; intro y r; apply h _ r
+
+  theorem L_reducible ty rho : Admissible rho -> Reducible (L ty rho) := by
+  sorry
+
+  theorem L_sn : Admissible rho -> L A rho t -> Term.SN t := by sorry
+
+  theorem L_var A K x : Admissible rho -> L A rho (.bound K x) := by sorry
+
+  theorem soundness : Γ ⊢ t : A -> ∀ f rho σ, Admissible rho -> EL Γ f rho σ -> L A rho ([σ]t) := by
+  intro j
+  induction j
+  case ax => sorry
+  case var => sorry
+  case pi => sorry
+  case tpi => sorry
+  case lam => sorry
+  case app => sorry
+  case econv => sorry
+  case iconv => sorry
+
+  theorem rho_id : Admissible (λ _ => Term.SN) := by
+  intro x; simp; apply reducible_sn
+
+  theorem type_L : Γ ⊢ t : A -> Admissible rho -> L A rho t := by
+  intro j h
+  have lem1 := ctx_wf j
+  cases lem1
+  case _ f lem1 =>
+    have lem := soundness j f rho I h
+    simp at lem; apply lem
+    intro x; simp
+    apply L_var _ _ _ h
+
+  theorem strong_normalization : Γ ⊢ t : A -> Term.SN t := by
+  intro j
+  apply L_sn; apply rho_id; apply type_L
+  apply j; apply rho_id
+
+end Fomega.Proof
