FomegaMut/Basic.lean
@@ -1,5 +1,0 @@
-
-import FomegaMut.Basic.Classification
-import FomegaMut.Basic.Inversion
-import FomegaMut.Basic.Substitution
-import FomegaMut.Basic.Weaken
