WCCC/Ctx.lean
@@ -1,28 +1,28 @@
 
 import Common
 
-namespace FomegaMut
+namespace WCCC
 
   abbrev Ctx := List Term
 
   @[simp]
   def nth : List Term -> Nat -> Term
-  | [], _ => ★
+  | [], _ => .none
   | .cons h _, 0 => h
   | .cons _ t, n + 1 => nth t n
 
   @[simp]
   def dnth : List Term -> Nat -> Term
-  | [], _ => ★
+  | [], _ => .none
   | .cons h _, 0 => [S]h
   | .cons _ t, n + 1 => [S](dnth t n)
 
-end FomegaMut
+end WCCC
 
-infix:1000 "@" => FomegaMut.nth
-infix:1000 "d@" => FomegaMut.dnth
+infix:1000 "@" => WCCC.nth
+infix:1000 "d@" => WCCC.dnth
 
-namespace FomegaMut
+namespace WCCC
 
   theorem dnth_as_nth : Γ d@ n = [Sn (n + 1)](Γ @ n) := by
   induction n generalizing Γ
@@ -33,4 +33,4 @@ namespace FomegaMut
     case _ A Γ =>
       rw [ih]; simp
 
-end FomegaMut
+end WCCC
